nsl/Security.ec
@@ -7,8 +7,8 @@ require Birthday.
 (* ------------------------------------------------------------------------------------------ *)
 
 (* AEAD Reduction *)
-module (Red_AEAD (D : A_GAKE) : A_GAEAD) (O : GAEAD_out) = {
-  module WAKE_O : GAKE_out = Game1 with {
+module (AEAD_Reduction (D : AKE_Adversary) : AEAD_Adversary) (O : AEAD_Oracles) = {
+  module R : AKE_Oracles_i = Game1a with {
     - var psk_map
     proc init_mem [ -1 - ]
     proc gen_pskey [ ^if ~ { O.gen(a, b); } ]
@@ -16,7 +16,10 @@ module (Red_AEAD (D : A_GAKE) : A_GAEAD) (O : GAEAD_out) = {
       var ex : bool
       ^if + ^ { ex <@ O.ex(a, b); }
       ^if ~ ((a, i) \notin state_map /\ ex)
-      [^if.^ca<$ - ^mo<-] ~ { mo <@ O.enc((a, b), msg1_data a b, na); }
+      ^if.^ca<$ ~ {
+        mo <@ O.enc((a, b), msg1_data a b, na);
+        ca <- oget mo;
+      }
     ]
     proc send_msg2 [
       var ex : bool
@@ -25,25 +28,31 @@ module (Red_AEAD (D : A_GAKE) : A_GAEAD) (O : GAEAD_out) = {
       ^if ~ ((b, j) \notin state_map /\ ex)
       ^if.^match + ^ { n <@ O.dec((a, b), msg1_data a b, ca); }
       ^if.^match ~ (n)
-      [^if.^match#Some.^cb<$ - ^mo<-] ~ { mo <@ O.enc((a, b), msg2_data a b ca, nb); }
+      ^if.^match#Some.^cb<$ ~ {
+        mo <@ O.enc((a, b), msg2_data a b ca, nb);
+        cb <- oget mo;
+      }
     ]
     proc send_msg3 [
       var n : nonce option
-      ^if.^match#IPending.^match + ^ { n <@ O.dec((a, b), msg2_data a b ca, m2); }
+      ^if.^match#IPending.^match + ^ { n <@ O.dec((m1.`1, b), msg2_data m1.`1 b m1.`2, m2); }
       ^if.^match#IPending.^match ~ (n)
-      [^if.^match#IPending.^match#Some.^caf<$ - ^mo<-] ~ { mo <@ O.enc((a, b), msg3_data a b ca m2, ok); }
+      ^if.^match#IPending.^match#Some.^cok<$ ~ {
+        mo <@ O.enc((m1.`1, b), msg3_data m1.`1 b m1.`2 m2, nok);
+        cok <- oget mo;
+      }
     ]
     proc send_fin [
       var n : nonce option
-      ^if.^match#RPending.^match + ^ { n <@ O.dec((a, b), msg3_data a b ca cb, m3); }
+      ^if.^match#RPending.^match + ^ { n <@ O.dec((m1.`1, b), msg3_data m1.`1 b m1.`2 m2, m3); }
       ^if.^match#RPending.^match ~ (n)
     ]
   }
 
   proc run(b) = {
     var b';
-    WAKE_O.init_mem(b);
-    b' <@ D(WAKE_O).run();
+    R.init_mem(b);
+    b' <@ D(R).run();
     return b';
   }
 }.
@@ -59,79 +68,75 @@ clone PROM.FullRO as NROc with
   type d_out_t <= bool
 proof *.
 
-module (Red_ROM (D : A_GAKE) : NROc.RO_Distinguisher) (O : NROc.RO) = {
-  module WAKE_O : GAKE_out = Game4 with {
+module (Nonce_Delay_Reduction (D : AKE_Adversary) : NROc.RO_Distinguisher) (O : NROc.RO) = {
+  module R : AKE_Oracles_i = Game3b with {
+    - var nonce_map
+    proc init_mem [ -1 - ]
     proc send_msg1 [
-      ^if.^if.^na<$ ~ {na <- witness; O.sample((msg1_data a b, ca)); }
+      [^if.^if.^na<$ - 1] ~ { O.sample((msg1_data a b, ca)); }
     ]
-
     proc send_msg2 [
-      ^if.^match#Some.^if.^nb<$ ~ {nb <- witness; O.sample((msg2_data a b ca, cb)); }
+      [^if.^match#Some.^if.^nb<$ - 1] ~ { O.sample((msg2_data a b ca, cb)); }
     ]
-
     proc send_msg3 [
-      ^if.^match#IPending.^match#Some.^if.^ok<$ ~ {
-        ok <- witness;
-        O.sample((msg3_data a b ca m2, caf));
-      }
-      ^if.^match#IPending.^match#Some.^if.^skey<- ~ {
-        na <@ O.get((msg1_data a b, ca));
-        ok <@ O.get((msg2_data a b ca, m2));
-        skey <- prf (na, ok) (a, b);
+      var nb' : nonce
+      ^if.^match#IPending.^match#Some.^if.^k<- ~ {
+        na <@ O.get((msg1_data m1.`1 b, m1.`2));
+        nb' <@ O.get((msg2_data m1.`1 b m1.`2, m2));
+        k <- prf (na, nb') (m1.`1, b);
       }
     ]
-
     proc send_fin [
-      ^if.^match#RPending.^match#Some.^skey<- ~ {
-        na <@ O.get((msg1_data a b, ca));
-        nb <@ O.get((msg2_data a b ca, cb));
-        skey <- prf (na, nb) (a, b);
+      ^if.^match#RPending.^match#Some.^k<- ~ {
+        na <@ O.get((msg1_data m1.`1 b, m1.`2));
+        nb <@ O.get((msg2_data m1.`1 b m1.`2, m2));
+        k <- prf (na, nb) (m1.`1, b);
       }
     ]
   }
 
   proc distinguish(b) = {
     var b';
-    WAKE_O.init_mem(b);
-    b' <@ D(WAKE_O).run();
+    R.init_mem(b);
+    b' <@ D(R).run();
     return b';
   }
 }.
+
 (* ------------------------------------------------------------------------------------------ *)
 (* PRF Reduction *)
 
-module (Red_PRF (D : A_GAKE) : A_GPRF) (O : GPRF_out) = {
-  module WAKE_O : GAKE_out = Game5 with {
+module (PRF_Reduction (D : AKE_Adversary) : PRF_Adversary) (O : PRF_Oracles) = {
+  module R : AKE_Oracles_i = Game4 with {
     - var prfkey_map
-    proc init_mem [-1 -]
+    proc init_mem [ ^b0<- & +1 -]
     proc send_msg3 [
-      var skeyo : skey option
-      [^if.^match#IPending.^match#Some.^if.^ <$ - ^skey<-] ~ {
-        O.gen((msg3_data a b ca m2, caf));
-        skeyo <@ O.f((msg3_data a b ca m2, caf), (a, b));
-        skey <- oget skeyo;
+      var ko : skey option
+      [^if.^match#IPending.^match#Some.^if.^na<$ - ^k<-] ~ {
+        O.gen((msg3_data m1.`1 b m1.`2 m2, cok));
+        ko <@ O.f((msg3_data m1.`1 b m1.`2 m2, cok), (m1.`1, b));
+        k <- oget ko;
       }
     ]
-
     proc send_fin [
-      var skeyo : skey option
-      ^if.^match#RPending.^match#Some.^skey<- ~ {
-        skeyo <@ O.f((msg3_data a b ca cb, m3), (a, b));
-        skey <- oget skeyo;
+      var ko : skey option
+      ^if.^match#RPending.^match#Some.^k<- ~ {
+        ko <@ O.f((msg3_data m1.`1 b m1.`2 m2, m3), (m1.`1, b));
+        k <- oget ko;
       }
     ]
   }
 
   proc run(b) = {
     var b';
-    WAKE_O.init_mem(b);
-    b' <@ D(WAKE_O).run();
+    R.init_mem(b);
+    b' <@ D(R).run();
     return b';
   }
 }.
 
 (* ------------------------------------------------------------------------------------------ *)
-(* Ctxt Collision Reduction *)
+(* Ciphertext Collision Reduction *)
 
 op q_m1 : { int | 0 <= q_m1 } as ge0_q_m1.
 op q_m2 : { int | 0 <= q_m2 } as ge0_q_m2.
@@ -143,10 +148,10 @@ clone Birthday as BD with
   proof*.
 realize ge0_q by smt(ge0_q_m1 ge0_q_m2 ge0_q_m3).
 
-module Counter (W : GAKE_out) : GAKE_out_i = {
+module Counter (O : AKE_Oracles) : AKE_Oracles_i = {
   var cm1, cm2, cm3 : int
 
-  include W[send_fin, gen_pskey, test, reveal]
+  include O[send_fin, gen_pskey, test, reveal]
 
   proc init_mem(b: bool) = {
     (cm1, cm2, cm3) <- (0, 0, 0);
@@ -155,52 +160,42 @@ module Counter (W : GAKE_out) : GAKE_out_i = {
   proc send_msg1(x) = {
     var m;
     cm1 <- cm1 + 1;
-    m <@ W.send_msg1(x);
+    m <@ O.send_msg1(x);
     return m;
   }
   proc send_msg2(x) = {
     var m;
     cm2 <- cm2 + 1;
-    m <@ W.send_msg2(x);
+    m <@ O.send_msg2(x);
     return m;
   }
   proc send_msg3(x) = {
     var m;
     cm3 <- cm3 + 1;
-    m <@ W.send_msg3(x);
+    m <@ O.send_msg3(x);
     return m;
   }
 }.
 
-module Red_Coll_O_WAKE (S : BD.ASampler) = Game2 with {
-  proc send_msg1 [
-    ^if.^ca<$ ~ {ca <@ S.s();}
-  ]
-
-  proc send_msg2 [
-    ^if.^match#Some.^cb<$ ~ {cb <@ S.s();}
-  ]
-
-  proc send_msg3 [
-    ^if.^match#IPending.^match#Some.^caf<$ ~ { caf <@ S.s(); }
-  ]
+module Collision_Reduction_Oracles (O : BD.ASampler) = Game2 with {
+  proc send_msg1 [ ^if.^ca<$ ~ { ca <@ O.s(); } ]
+  proc send_msg2 [ ^if.^match#Some.^cb<$ ~ { cb <@ O.s(); } ]
+  proc send_msg3 [ ^if.^match#IPending.^match#Some.^cok<$ ~ { cok <@ O.s(); } ]
 }.
 
-module (Red_Coll_real (A : A_GAKE) : BD.Adv) (S : BD.ASampler) = {
+module (Collision_Reduction_0 (A : AKE_Adversary) : BD.Adv) (O : BD.ASampler) = {
   proc a() = {
-    var b;
-    Red_Coll_O_WAKE(S).init_mem(false);
-    Counter(Red_Coll_O_WAKE(S)).init_mem(false);
-    b <@ A(Counter(Red_Coll_O_WAKE(S))).run();
+    Collision_Reduction_Oracles(O).init_mem(false);
+    Counter(Collision_Reduction_Oracles(O)).init_mem(false);
+    A(Counter(Collision_Reduction_Oracles(O))).run();
   }
 }.
 
-module (Red_Coll_ideal (A : A_GAKE) : BD.Adv) (S : BD.ASampler) = {
+module (Collision_Reduction_1 (A : AKE_Adversary) : BD.Adv) (O : BD.ASampler) = {
   proc a() = {
-    var b;
-    Red_Coll_O_WAKE(S).init_mem(true);
-    Counter(Red_Coll_O_WAKE(S)).init_mem(true);
-    b <@ A(Counter(Red_Coll_O_WAKE(S))).run();
+    Collision_Reduction_Oracles(O).init_mem(true);
+    Counter(Collision_Reduction_Oracles(O)).init_mem(true);
+    A(Counter(Collision_Reduction_Oracles(O))).run();
   }
 }.
 
@@ -215,33 +210,33 @@ clone PROM.FullRO as KROc with
   type d_out_t <= bool
 proof *.
 
-module (Red_ROM_sk (D : A_GAKE) : KROc.RO_Distinguisher) (R : KROc.RO) = {
-  module WAKE_O : GAKE_out = Game8 with {
-    - var sk_map
-
-    proc init_mem [
-      -1 -
-    ]
-
-    proc send_msg3 [
-      ^if.^match#IPending.^match#Some.^if.^skey<- + ^ {
-        R.sample(((a, ca), m2, caf));
+module (Key_Delay_Reduction (D : AKE_Adversary) : KROc.RO_Distinguisher) (O : KROc.RO) = {
+  module R : AKE_Oracles_i = Game5a with {
+    proc init_mem [ -1 - ]
+    proc send_msg3 [ ^if.^match#IPending.^match#Some.^if.^k<- + ^ { O.sample((m1, m2, cok)); } ]
+    proc reveal [
+      var k' : skey
+      ^if.^match#Accepted.^if.1 ~ {
+        k' <@ O.get(t);
+        ko <- Some k';
       }
     ]
-
-    proc reveal [
-      [^if.^match#Accepted.^if.^k''<$ - ^k<-] ~ { k <@ R.get(trace); }
-    ]
-
     proc test [
-      [^if.^match#Accepted.^if.^k''<$ - ^if{2}] ~ { k <@ R.get(trace); if (b0) k <$ dskey; }
+      ^if.^match#Accepted.^if.1 ~ {
+        k' <@ O.get(t);
+        if (b0 = false) {
+          k' <- k';
+        } else {
+          k' <$ dskey;
+        }
+      }
     ]
   }
 
   proc distinguish(b) = {
     var b';
-    WAKE_O.init_mem(b);
-    b' <@ D(WAKE_O).run();
+    R.init_mem(b);
+    b' <@ D(R).run();
     return b';
   }
 }.
@@ -251,301 +246,347 @@ module (Red_ROM_sk (D : A_GAKE) : KROc.RO_Distinguisher) (R : KROc.RO) = {
 (* ------------------------------------------------------------------------------------------ *)
 section.
 
-declare module A <: A_GAKE {-GAKEb, -Game1, -Game2, -Game3, -Game4, -Game4', -Game5, -Game6, -Game7, -Game8, -GAEAD0, -GAEAD1, -PRF0, -PRF1, -Red_AEAD, -Red_Coll_real, -Red_Coll_ideal, -Red_ROM, -Red_PRF, -NROc.RO, -NROc.FRO, -BD.Sample, -KROc.RO, -KROc.FRO, -Red_ROM_sk}.
+declare module A <: AKE_Adversary {
+  -AKE_Oracles,
+  -AEAD_Oracles_0, -AEAD_Oracles_1,
+  -PRF_Oracles_0, -PRF_Oracles_1,
+  -AEAD_Reduction, -PRF_Reduction,
+  -Nonce_Delay_Reduction, -NROc.RO, -NROc.FRO,
+  -Key_Delay_Reduction, -KROc.RO, -KROc.FRO,
+  -Collision_Reduction_0, -Collision_Reduction_1, -BD.Sample,
+  -Game1, -Game1a,
+  -Game2,
+  -Game3, -Game3a, -Game3b, -Game3c, -Game3d,
+  -Game4,
+  -Game5, -Game5a, -Game5b, -Game5c
+}.
 
 declare axiom A_ll:
-forall (GW <: GAKE_out{-A}),
-  islossless GW.gen_pskey =>
-  islossless GW.send_msg1 =>
-  islossless GW.send_msg2 =>
-  islossless GW.send_msg3 =>
-  islossless GW.send_fin =>
-  islossless GW.reveal => islossless GW.test => islossless A(GW).run.
+  forall (O <: AKE_Oracles { -A }),
+  islossless O.gen_pskey =>
+  islossless O.send_msg1 =>
+  islossless O.send_msg2 =>
+  islossless O.send_msg3 =>
+  islossless O.send_fin =>
+  islossless O.reveal =>
+  islossless O.test =>
+  islossless A(O).run.
 
-declare axiom A_bounded_qs: forall (GW <: GAKE_out{-A}), hoare[A(Counter(GW)).run: Counter.cm1 = 0 /\ Counter.cm2 = 0 /\ Counter.cm3 = 0 ==> Counter.cm1 <= q_m1 /\ Counter.cm2 <= q_m2 /\ Counter.cm3 <= q_m3].
+declare axiom A_bounded_qs:
+  forall (O <: AKE_Oracles { -A }),
+  hoare[A(Counter(O)).run:
+        Counter.cm1 = 0 /\ Counter.cm2 = 0 /\ Counter.cm3 = 0
+    ==> Counter.cm1 <= q_m1 /\ Counter.cm2 <= q_m2 /\ Counter.cm3 <= q_m3
+  ].
 
 (* ------------------------------------------------------------------------------------------ *)
-(* Step 0: Inline procedure calls, and remove pskeys from the state using psk_map to retrieve. *)
+(* Hop 1: AKE Game to Game 1 - Inline procedure calls *) 
+  
+lemma Hop1 bit &m:
+    Pr[AKE_Game(AKE_Oracles(NSL), A).run(bit) @ &m : res] = Pr[AKE_Game(Game1, A).run(bit) @ &m : res].
+proof.
+byequiv => //.
+proc; inline.
+call (: ={b0, state_map, psk_map}(AKE_Oracles, Game1) ).
++ by sim.
++ proc; inline.
+  sp; if => //.
+  by auto.
++ proc; inline.
+  sp; if => //.
+  sp; match = => //.
+  + match None {1} ^match; 1: by auto.
+    by auto.
+  move => na.
+  match Some {1} ^match; 1: by auto => /#.
+  by auto.
++ proc; inline.
+  sp; if => //.
+  sp; match =; try by auto.
+  + smt().
+  move => si m1.
+  sp; match = => //.
+  + match None {1} ^match; 1: by auto.
+    by auto.
+  move => nb.
+  match Some {1} ^match; 1: by auto => /#.
+  by auto.
++ proc; inline.
+  sp; if => //.
+  sp; match =; try by auto.
+  + smt().
+  move => sr m1 m2.
+  sp; match = => //.
+  + match None {1} ^match; 1: by auto.
+    by auto.
+  move => nok.
+  match Some {1} ^match; 1: by auto => /#.
+  by auto.
++ by sim.
++ by sim.
+by auto.
+qed.
 
-local op clear_psk (s : instance_state) =
+(* ------------------------------------------------------------------------------------------ *)
+(* Hop 2: Game 1 to Game 1a - cleanup session state redundancies *) 
+
+local op clean1 (s : session_state) =
 match s with
 | IPending st m1 =>
-  let (id, psk, na, ca) = st in IPending (id, witness, na, ca) m1
+  let (id, psk, na, ca) = st in IPending (id, witness, na, witness) m1
 | RPending st m1 m2 =>
-  let (id, psk, na, nb, ca, cb) = st in RPending (id, witness, na, nb, ca, cb) m1 m2
+  let (id, psk, na, nb, ca, cb) = st in RPending (witness, witness, na, nb, witness, witness) m1 m2
 | Accepted _ _ => s
 | Observed _ _ => s
 | Aborted   => s
 end.
 
-local lemma eq_partners tr r sml smr:
-  (forall h, omap (fun (v: role * instance_state) => let (r, s) = v in (r, clear_psk s)) sml.[h] = smr.[h]) =>
-get_partners tr r sml = get_partners tr r smr.
+local lemma clean1_fresh h sml smr:
+  (forall h, omap (fun (v: _ * _) => let (r, s) = v in (r, clean1 s)) sml.[h] = smr.[h]) =>
+  fresh h sml <=> fresh h smr.
 proof.
-move=> eqsm.
-rewrite /get_partners.
-congr.
-apply fmap_eqP => h'.
-rewrite !filterE -(eqsm h') /=.
-case: (sml.[h'])=> //=.
-by move=> [r' []] // [] /= /#.
+move=> eq_sm.
+rewrite /fresh.
+have eq_ps : partners h sml = partners h smr.
++ rewrite /partners.
+  congr.
+  apply fmap_eqP => h'.
+  rewrite !filterE -(eq_sm h') /=.
+  by case: (sml.[h']); smt().
+rewrite /observed_partners eq_ps.
+do! congr.
+rewrite fun_ext => h'.
+rewrite -(eq_sm h') //=.
+case: (sml.[h'])=> //.
+by move => [r' []] // [].
 qed.
 
-local lemma eq_obs_partners h sml smr:
-  (forall h, omap (fun (v: role * instance_state) => let (r, s) = v in (r, clear_psk s)) sml.[h] = smr.[h]) =>
-get_observed_partners h sml = get_observed_partners h smr.
-proof.
-move=> eqsm.
-rewrite /get_observed_partners.
-congr.
-+ rewrite fun_ext => bj.
-  rewrite -(eqsm bj) //=.
-  case: (sml.[bj])=> //.
-  by move=> [r' []] // [].
-rewrite -(eq_partners _ _ sml smr eqsm).
-rewrite -(eqsm h) /s /r //=.
-case: (sml.[h])=> //.
-by move=> [r' []] // [].
-qed.
-
-lemma Step0 bit &m:
-    Pr[E_GAKE(GAKEb(NSL), A).run(bit) @ &m : res] = Pr[E_GAKE(Game1, A).run(bit) @ &m : res].
+lemma Hop2 bit &m:
+    Pr[AKE_Game(Game1, A).run(bit) @ &m : res] = Pr[AKE_Game(Game1a, A).run(bit) @ &m : res].
 proof.
 byequiv => //.
 proc; inline*.
 call (:
-    ={b0, psk_map}(GAKEb, Game1)
-/\ (forall h, omap (fun v => let (r, s) = v in (r, clear_psk s)) GAKEb.state_map.[h]{1} = Game1.state_map.[h]{2})
-/\ (forall a i, GAKEb_inv GAKEb.state_map GAKEb.psk_map a i){1}
+    ={b0, psk_map}(Game1, Game1a)
+/\ (forall h, omap (fun v => let (r, s) = v in (r, clean1 s)) Game1.state_map.[h]{1} = Game1a.state_map.[h]{2})
+/\ (forall a i, Game1_inv Game1.state_map Game1.psk_map a i){1}
 ).
 - conseq (: ={res}
-          /\ ={b0, psk_map}(GAKEb, Game1)
-          /\ (forall h, omap (fun v => let (r, s) = v in (r, clear_psk s)) GAKEb.state_map.[h]{1} = Game1.state_map.[h]{2})
-  ) GAKEb_inv_gen_pskey _ => //.
+          /\ ={b0, psk_map}(Game1, Game1a)
+          /\ (forall h, omap (fun v => let (r, s) = v in (r, clean1 s)) Game1.state_map.[h]{1} = Game1a.state_map.[h]{2})
+  ) Game1_inv_gen_pskey _ => //.
   proc.
   by if; auto.
 
 - conseq (: ={res}
-          /\ ={b0, psk_map}(GAKEb, Game1)
-          /\ (forall h, omap (fun v => let (r, s) = v in (r, clear_psk s)) GAKEb.state_map.[h]{1} = Game1.state_map.[h]{2})
-  ) GAKEb_inv_send_msg1 _ => //.
+          /\ ={b0, psk_map}(Game1, Game1a)
+          /\ (forall h, omap (fun v => let (r, s) = v in (r, clean1 s)) Game1.state_map.[h]{1} = Game1a.state_map.[h]{2})
+  ) Game1_inv_send_msg1 _ => //.
   proc; inline.
-  sp; wp; if=> //.
+  sp; wp; if => //.
   + smt().
-  auto=> />.
+  auto => />.
   smt(get_setE).
 
 - conseq (: ={res}
-          /\ ={b0, psk_map}(GAKEb, Game1)
-          /\ (forall h, omap (fun v => let (r, s) = v in (r, clear_psk s)) GAKEb.state_map.[h]{1} = Game1.state_map.[h]{2})
-  ) GAKEb_inv_send_msg2 _ => //.
+          /\ ={b0, psk_map}(Game1, Game1a)
+          /\ (forall h, omap (fun v => let (r, s) = v in (r, clean1 s)) Game1.state_map.[h]{1} = Game1a.state_map.[h]{2})
+  ) Game1_inv_send_msg2 _ => //.
   proc; inline.
-  sp; wp; if=> //.
+  sp; wp; if => //.
   + smt().
   sp; match =.
   + smt().
-  + auto=> />.
+  + auto => />.
     smt(get_setE).
-  move=> na.
-  by match Some {1} ^match; auto; smt(get_setE).
+  by auto; smt(get_setE).
 
 - conseq (: ={res}
-          /\ ={b0, psk_map}(GAKEb, Game1)
-          /\ (forall h, omap (fun v => let (r, s) = v in (r, clear_psk s)) GAKEb.state_map.[h]{1} = Game1.state_map.[h]{2})
-  ) GAKEb_inv_send_msg3 _ => //.
+          /\ ={b0, psk_map}(Game1, Game1a)
+          /\ (forall h, omap (fun v => let (r, s) = v in (r, clean1 s)) Game1.state_map.[h]{1} = Game1a.state_map.[h]{2})
+  ) Game1_inv_send_msg3 _ => //.
   proc; inline.
-  sp; wp; if=> //.
+  sp; wp; if => //.
   + smt().
   sp; match; 1..5: (
-    move=> &1 &2 /> + + /(_ (a, i){2});
+    move => &1 &2 /> + + /(_ (a, i){2});
     rewrite domE;
-    case: (GAKEb.state_map{1}.[(a, i)]{2})=> />;
-    move=> + H;
+    case: (Game1.state_map{1}.[a, i]{2})=> />;
+    move => + H;
     by rewrite -H => /#
-  ); 2..5: by auto.
-  move=> sil m1l sir m1r.
+  ); ~1: by auto.
+  move => sil m1l sir m1r.
   sp; match =.
-  + auto=> />.
+  + auto => />.
     smt(get_setE).
-  + match None {1} ^match; 1: by auto.
-    auto => />.
-    move=> &1 &2 _ _ smr sml inv_sm invl aiin sms.
-    smt(get_setE).
-  move=> nb.
-  match Some {1} ^match.
-  + auto; smt(get_setE).
-  auto=> />.
-  move=> &1 &2 + + + sml + invl.
+  + by auto; smt(get_setE).
+  auto => />.
   smt(get_setE).
 
 - conseq (: ={res}
-          /\ ={b0, psk_map}(GAKEb, Game1)
-          /\ (forall h, omap (fun v => let (r, s) = v in (r, clear_psk s)) GAKEb.state_map.[h]{1} = Game1.state_map.[h]{2})
-  ) GAKEb_inv_send_fin _ => //.
+          /\ ={b0, psk_map}(Game1, Game1a)
+          /\ (forall h, omap (fun v => let (r, s) = v in (r, clean1 s)) Game1.state_map.[h]{1} = Game1a.state_map.[h]{2})
+  ) Game1_inv_send_fin _ => //.
   proc; inline.
-  sp; wp ^if ^if; if=> //.
+  sp; wp ^if ^if; if => //.
   + smt().
   sp; match; 1..5: (
-    move=> &1 &2 /> + + /(_ (b, j){2});
+    move => &1 &2 /> + + /(_ (b, j){2});
     rewrite domE;
-    case: (GAKEb.state_map{1}.[(b, j)]{2})=> />;
-    move=> + H;
+    case: (Game1.state_map{1}.[b, j]{2}) => />;
+    move => + H;
     by rewrite -H /#
-  ); 1,3,4,5: by auto.
-  move=> sil m1l m2l sir m1r m2r.
+  ); ~2: by auto.
+  move => sil m1l m2l sir m1r m2r.
   sp; match =.
-  + auto=> />.
+  + auto => />.
     smt().
-  + match None {1} ^match; 1: by auto.
-    auto=> />.
+  + auto => />.
     smt(get_setE).
-  move=> nb.
-  match Some {1} ^match.
-  + auto; smt(get_setE).
-  auto=> />.
+  auto => />.
   smt(get_setE).
 
 - conseq (: ={res}
-          /\ ={b0, psk_map}(GAKEb, Game1)
-          /\ (forall h, omap (fun v => let (r, s) = v in (r, clear_psk s)) GAKEb.state_map.[h]{1} = Game1.state_map.[h]{2})
-  ) GAKEb_inv_reveal _ => //.
+          /\ ={b0, psk_map}(Game1, Game1a)
+          /\ (forall h, omap (fun v => let (r, s) = v in (r, clean1 s)) Game1.state_map.[h]{1} = Game1a.state_map.[h]{2})
+  ) Game1_inv_reveal _ => //.
   proc; inline.
   sp; wp ^if ^if; if=> //.
   + smt().
   sp; match; 1..5:(
-    move=> &1 &2 /> + + /(_ (a, i){2});
+    move => &1 &2 /> + + /(_ h{2});
     rewrite domE;
-    case: (GAKEb.state_map{1}.[(a, i)]{2})=> />;
-    move=> + H;
+    case: (Game1.state_map{1}.[h]{2}) => />;
+    move => + H;
     by rewrite -H => /#
-  ); 1,2,4,5: by auto.
-  move=> tr k tr' k'.
-  sp ^if & -1 ^if & -1; if=> //.
-  + move => &1 &2 [] /> *.
-    by rewrite (eq_obs_partners (a, i){2} GAKEb.state_map{1} Game1.state_map{2}) => //.
-  auto=> /> &1 &2 + + eqsm invl a_in _.
-  rewrite -(eqsm (a, i){2}).
+  ); ~3: by auto.
+  move => tr k tr' k'.
+  if => //.
+  + move => &1 &2 |> *.
+    by rewrite (clean1_fresh h{2} Game1.state_map{1} Game1a.state_map{2}).
+  auto => /> &1 &2 + + eq_sm invl a_in _.
+  rewrite -(eq_sm h{2}).
   move => *.
-  split. smt().
-  move => h.
-  case (h = (a, i){2}) => [|hneq].
+  split; 1: smt().
+  move => h'.
+  case (h' = h{2}) => [|hneq].
   + smt(get_set_sameE).
-  do rewrite get_set_neqE => //.
-  by rewrite eqsm.
+  rewrite !get_set_neqE //.
+  by rewrite eq_sm.
 
 - conseq (: ={res}
-          /\ ={b0, psk_map}(GAKEb, Game1)
-          /\ (forall h, omap (fun v => let (r, s) = v in (r, clear_psk s)) GAKEb.state_map.[h]{1} = Game1.state_map.[h]{2})
-     ) GAKEb_inv_test _ => //.
+          /\ ={b0, psk_map}(Game1, Game1a)
+          /\ (forall h, omap (fun v => let (r, s) = v in (r, clean1 s)) Game1.state_map.[h]{1} = Game1a.state_map.[h]{2})
+     ) Game1_inv_test _ => //.
   proc; inline.
   sp; wp ^if ^if; if=> //.
   + smt().
   sp; match; 1..5:(
-    move=> &1 &2 /> + + /(_ (a, i){2});
+    move => &1 &2 /> + + /(_ h{2});
     rewrite domE;
-    case: (GAKEb.state_map{1}.[(a, i)]{2})=> />;
-    move=> + H;
+    case: (Game1.state_map{1}.[h]{2}) => />;
+    move => + H;
     by rewrite -H => /#
-  ); 1,2,4,5: by auto.
-  move=> tr k tr' k'.
-  sp ^if & -1 ^if & -1; if=> //.
-  + move => &1 &2 [] /> *.
-    by rewrite (eq_obs_partners (a, i){2} GAKEb.state_map{1} Game1.state_map{2}) => //.
+  ); ~3: by auto.
+  move => tr k tr' k'.
   if => //.
-  + auto=> /> &1 &2 + + eqsm invl a_in _.
-    rewrite -(eqsm (a, i){2}).
+  + move => &1 &2 |> *.
+    by rewrite (clean1_fresh h{2} Game1.state_map{1} Game1a.state_map{2}).
+  if => //.
+  - auto => /> &1 &2 + + eq_sm invl a_in _.
+    rewrite -(eq_sm h{2}).
     move => *.
-    split. smt().
-    move => h.
-    case (h = (a, i){2}) => [|hneq].
+    split; 1: smt().
+    move => h'.
+    case (h' = h{2}) => [|hneq].
     + smt(get_set_sameE).
-    do rewrite get_set_neqE => //.
-    by rewrite eqsm.
-  auto=> /> &1 &2 + + eqsm invl _ a_in _ ideal sk _.
-  rewrite -(eqsm (a, i){2}).
-  move => stm1 stm2 h.
-  case (h = (a, i){2}) => [|hneq].
+    rewrite !get_set_neqE //.
+    by rewrite eq_sm.
+  auto => /> &1 &2 + + eq_sm invl a_in _.
+  rewrite -(eq_sm h{2}).
+  move => 7? h'.
+  case (h' = h{2}) => [|hneq].
   + smt(get_set_sameE).
-  do rewrite get_set_neqE => //.
-  by rewrite eqsm.
+  rewrite !get_set_neqE //.
+  by rewrite eq_sm.
 
 auto=> />.
 smt(emptyE).
 qed.
 
 (* ------------------------------------------------------------------------------------------ *)
-(* Step 1: Apply the AEAD assumption. *)
+(* Game 1a to Game 2 - Apply the AEAD assumption. *)
 
-lemma Step1 bit &m:
-    `|Pr[E_GAKE(Game1, A).run(bit) @ &m : res] - Pr[E_GAKE(Game2, A).run(bit) @ &m : res]|
+lemma Hop3 bit &m:
+    `|Pr[AKE_Game(Game1a, A).run(bit) @ &m : res] - Pr[AKE_Game(Game2, A).run(bit) @ &m : res]|
   =
-    `|Pr[E_GAEAD(GAEAD0, Red_AEAD(A)).run(bit) @ &m : res] - Pr[E_GAEAD(GAEAD1, Red_AEAD(A)).run(bit) @ &m : res]|.
+    `|Pr[AEAD_Game(AEAD_Oracles_0, AEAD_Reduction(A)).run(bit) @ &m : res] - Pr[AEAD_Game(AEAD_Oracles_1, AEAD_Reduction(A)).run(bit) @ &m : res]|.
 proof.
 do! congr.
 + byequiv => //.
   proc; inline*.
   wp.
   call (:
-        ={psk_map}(Game1, GAEADb)
-     /\ ={b0, state_map}(Game1, Red_AEAD.WAKE_O)
-     /\ (forall a i, Game1_inv Game1.state_map Game1.psk_map a i){1}
-  )=> //.
+        ={b0, state_map}(Game1a, AEAD_Reduction.R)
+     /\ Game1a.psk_map{1} = AEAD_Oracles_common.key_map{2}
+     /\ (forall a i, Game1a_inv Game1a.state_map Game1a.psk_map a i){1}
+  ) => //.
 
   - conseq (: ={res}
-         /\ ={psk_map}(Game1, GAEADb)
-         /\ ={b0, state_map}(Game1, Red_AEAD.WAKE_O)
-    ) Game1_inv_gen_pskey _ => //.
+         /\ ={b0, state_map}(Game1a, AEAD_Reduction.R)
+         /\ Game1a.psk_map{1} = AEAD_Oracles_common.key_map{2}
+    ) Game1a_inv_gen_pskey _ => //.
     by proc; inline; sp; if; auto.
 
   - conseq (: ={res}
-         /\ ={psk_map}(Game1, GAEADb)
-         /\ ={b0, state_map}(Game1, Red_AEAD.WAKE_O)
-    ) Game1_inv_send_msg1 _ => //.
+         /\ ={b0, state_map}(Game1a, AEAD_Reduction.R)
+         /\ Game1a.psk_map{1} = AEAD_Oracles_common.key_map{2}
+    ) Game1a_inv_send_msg1 _ => //.
     proc; inline.
-    sp; wp; if=> //.
+    sp; wp; if => //.
     by match Some {2} ^match; auto; smt().
 
   - conseq (: ={res}
-         /\ ={psk_map}(Game1, GAEADb)
-         /\ ={b0, state_map}(Game1, Red_AEAD.WAKE_O)
-    ) Game1_inv_send_msg2 _ => //.
+         /\ ={b0, state_map}(Game1a, AEAD_Reduction.R)
+         /\ Game1a.psk_map{1} = AEAD_Oracles_common.key_map{2}
+    ) Game1a_inv_send_msg2 _ => //.
     proc; inline.
-    sp; wp; if=> //.
+    sp; wp; if => //.
     match Some {2} ^match.
     + auto; smt().
     sp; match =.
-    + by move=> /> /#.
+    + by move => /> /#.
     + by auto.
-    move=> na.
+    move => na.
     by match Some {2} ^match; auto; smt().
 
   - conseq (: ={res}
-         /\ ={psk_map}(Game1, GAEADb)
-         /\ ={b0, state_map}(Game1, Red_AEAD.WAKE_O)
-    ) Game1_inv_send_msg3 _ => //.
+         /\ ={b0, state_map}(Game1a, AEAD_Reduction.R)
+         /\ Game1a.psk_map{1} = AEAD_Oracles_common.key_map{2}
+    ) Game1a_inv_send_msg3 _ => //.
     proc; inline.
     sp; wp; if=> //.
     sp; match = => //.
     + smt().
     move=> st m1.
-    exlim Game1.state_map{1}, Game1.psk_map{1}, a{1}, i{1} => sm pm a i.
-    case @[ambient] _: (forall a i, Game1_inv sm pm a i) => [inv|?]; 2: by exfalso => /#.
+    exlim Game1a.state_map{1}, Game1a.psk_map{1}, a{1}, i{1} => sm pm a i.
+    case @[ambient] _: (forall a i, Game1a_inv sm pm a i) => [inv|?]; 2: by exfalso => /#.
     match Some {2} ^match.
     + auto => />.
       smt(get_setE).
     sp; match =.
-    + by auto=> /> /#.
-    + by auto=> /> /#.
-    move=> nb.
+    + by auto => /> /#.
+    + by auto => /> /#.
+    move => nb.
     match Some {2} ^match.
     + auto => />.
       smt(get_setE).
-    by auto=> /> /#.
+    by auto => /> /#.
 
   - conseq (: ={res}
-         /\ ={psk_map}(Game1, GAEADb)
-         /\ ={b0, state_map}(Game1, Red_AEAD.WAKE_O)
-    ) Game1_inv_send_fin _ => //.
+         /\ ={b0, state_map}(Game1a, AEAD_Reduction.R)
+         /\ Game1a.psk_map{1} = AEAD_Oracles_common.key_map{2}
+    ) Game1a_inv_send_fin _ => //.
     proc; inline.
     sp; wp ^if ^if; if=> //.
     sp; match = => //.
@@ -557,240 +598,259 @@ do! congr.
     by sp; match =; auto=> /> /#.
 
   - conseq (: ={res}
-         /\ ={psk_map}(Game1, GAEADb)
-         /\ ={b0, state_map}(Game1, Red_AEAD.WAKE_O)
-    ) Game1_inv_reveal _ => //.
+         /\ ={b0, state_map}(Game1a, AEAD_Reduction.R)
+         /\ Game1a.psk_map{1} = AEAD_Oracles_common.key_map{2}
+    ) Game1a_inv_reveal _ => //.
     by sim.
 
   - conseq (: ={res}
-         /\ ={psk_map}(Game1, GAEADb)
-         /\ ={b0, state_map}(Game1, Red_AEAD.WAKE_O)
-    ) Game1_inv_test _ => //.
+         /\ ={b0, state_map}(Game1a, AEAD_Reduction.R)
+         /\ Game1a.psk_map{1} = AEAD_Oracles_common.key_map{2}
+    ) Game1a_inv_test _ => //.
     by sim.
 
-  auto=> />.
+  auto => />.
   smt(emptyE).
 
 byequiv => //.
 proc; inline*.
 wp.
 call (:
-      ={psk_map}(Game2, GAEADb)
-      /\ ={b0, state_map}(Game2, Red_AEAD.WAKE_O)
-      /\ Game2.dec_map{1} = GAEAD1.ctxts{2}
-      /\ (forall a i, Game1_inv Game2.state_map Game2.psk_map a i){1}
+         ={b0, state_map}(Game2, AEAD_Reduction.R)
+      /\ Game2.psk_map{1} = AEAD_Oracles_common.key_map{2}
+      /\ (forall a b m1, Game2.dec_map{1}.[msg1_data a b, m1] = AEAD_Oracles_1.dec_map{2}.[(a, b), msg1_data a b, m1])
+      /\ (forall a b m1 m2, Game2.dec_map{1}.[msg2_data a b m1, m2] = AEAD_Oracles_1.dec_map{2}.[(a, b), msg2_data a b m1, m2])
+      /\ (forall a b m1 m2 m3, Game2.dec_map{1}.[msg3_data a b m1 m2, m3] = AEAD_Oracles_1.dec_map{2}.[(a, b), msg3_data a b m1 m2, m3])
+      /\ (forall a i, Game1a_inv Game2.state_map Game2.psk_map a i){1}
 ).
 - conseq (: ={res}
-       /\ ={psk_map}(Game2, GAEADb)
-       /\ ={b0, state_map}(Game2, Red_AEAD.WAKE_O)
-       /\ Game2.dec_map{1} = GAEAD1.ctxts{2}
+         /\ ={b0, state_map}(Game2, AEAD_Reduction.R)
+         /\ Game2.psk_map{1} = AEAD_Oracles_common.key_map{2}
+         /\ (forall a b m1, Game2.dec_map{1}.[msg1_data a b, m1] = AEAD_Oracles_1.dec_map{2}.[(a, b), msg1_data a b, m1])
+         /\ (forall a b m1 m2, Game2.dec_map{1}.[msg2_data a b m1, m2] = AEAD_Oracles_1.dec_map{2}.[(a, b), msg2_data a b m1, m2])
+         /\ (forall a b m1 m2 m3, Game2.dec_map{1}.[msg3_data a b m1 m2, m3] = AEAD_Oracles_1.dec_map{2}.[(a, b), msg3_data a b m1 m2, m3])
   ) Game2_inv_gen_pskey _ => //.
   proc; inline; sp.
   by if; auto.
 
 - conseq (: ={res}
-       /\ ={psk_map}(Game2, GAEADb)
-       /\ ={b0, state_map}(Game2, Red_AEAD.WAKE_O)
-       /\ Game2.dec_map{1} = GAEAD1.ctxts{2}
+         /\ ={b0, state_map}(Game2, AEAD_Reduction.R)
+         /\ Game2.psk_map{1} = AEAD_Oracles_common.key_map{2}
+         /\ (forall a b m1, Game2.dec_map{1}.[msg1_data a b, m1] = AEAD_Oracles_1.dec_map{2}.[(a, b), msg1_data a b, m1])
+         /\ (forall a b m1 m2, Game2.dec_map{1}.[msg2_data a b m1, m2] = AEAD_Oracles_1.dec_map{2}.[(a, b), msg2_data a b m1, m2])
+         /\ (forall a b m1 m2 m3, Game2.dec_map{1}.[msg3_data a b m1 m2, m3] = AEAD_Oracles_1.dec_map{2}.[(a, b), msg3_data a b m1 m2, m3])
   ) Game2_inv_send_msg1 _ => //.
   proc; inline.
-  sp; wp; if=> //.
+  sp; wp; if => //.
   rcondt{2} ^if; 1: by auto.
   swap {2} ^c<$ @ ^na<$.
-  by auto.
+  auto => />.
+  smt(get_setE).
 
 - conseq (: ={res}
-       /\ ={psk_map}(Game2, GAEADb)
-       /\ ={b0, state_map}(Game2, Red_AEAD.WAKE_O)
-       /\ Game2.dec_map{1} = GAEAD1.ctxts{2}
+         /\ ={b0, state_map}(Game2, AEAD_Reduction.R)
+         /\ Game2.psk_map{1} = AEAD_Oracles_common.key_map{2}
+         /\ (forall a b m1, Game2.dec_map{1}.[msg1_data a b, m1] = AEAD_Oracles_1.dec_map{2}.[(a, b), msg1_data a b, m1])
+         /\ (forall a b m1 m2, Game2.dec_map{1}.[msg2_data a b m1, m2] = AEAD_Oracles_1.dec_map{2}.[(a, b), msg2_data a b m1, m2])
+         /\ (forall a b m1 m2 m3, Game2.dec_map{1}.[msg3_data a b m1 m2, m3] = AEAD_Oracles_1.dec_map{2}.[(a, b), msg3_data a b m1 m2, m3])
   ) Game2_inv_send_msg2 _ => //.
   proc; inline.
-  sp; wp; if=> //.
+  sp; wp; if => //.
   rcondt {2} 5; 1: by auto.
-  sp; match = => //.
+  sp; match =.
+  + smt().
   + by auto.
   move=> na.
   rcondt {2} ^if; 1: by auto.
   swap {2} ^c0<$ @ ^nb<$.
-  by auto.
+  auto => />.
+  smt(get_setE).
 
 - conseq (: ={res}
-       /\ ={psk_map}(Game2, GAEADb)
-       /\ ={b0, state_map}(Game2, Red_AEAD.WAKE_O)
-       /\ Game2.dec_map{1} = GAEAD1.ctxts{2}
+         /\ ={b0, state_map}(Game2, AEAD_Reduction.R)
+         /\ Game2.psk_map{1} = AEAD_Oracles_common.key_map{2}
+         /\ (forall a b m1, Game2.dec_map{1}.[msg1_data a b, m1] = AEAD_Oracles_1.dec_map{2}.[(a, b), msg1_data a b, m1])
+         /\ (forall a b m1 m2, Game2.dec_map{1}.[msg2_data a b m1, m2] = AEAD_Oracles_1.dec_map{2}.[(a, b), msg2_data a b m1, m2])
+         /\ (forall a b m1 m2 m3, Game2.dec_map{1}.[msg3_data a b m1 m2, m3] = AEAD_Oracles_1.dec_map{2}.[(a, b), msg3_data a b m1 m2, m3])
   ) Game2_inv_send_msg3 _ => //.
   proc; inline.
-  sp; wp; if=> //.
+  sp; wp; if => //.
   sp; match = => //.
   + smt().
   move=> st m1.
   rcondt {2} ^if.
-  + auto=> />.
+  + auto => />.
     smt(get_setE).
   sp; match =.
+  + smt().
   + by auto.
-  + by auto.
-  move=> nb.
+  move => nb.
   rcondt {2} ^if.
-  + auto=> />.
+  + auto => />.
     smt(get_setE).
-  swap {2} ^c0<$ @ ^ok<$.
-  by auto.
+  swap {2} ^c0<$ @ ^nok<$.
+  auto => />.
+  smt(get_setE).
 
 - conseq (: ={res}
-       /\ ={psk_map}(Game2, GAEADb)
-       /\ ={b0, state_map}(Game2, Red_AEAD.WAKE_O)
-       /\ Game2.dec_map{1} = GAEAD1.ctxts{2}
+         /\ ={b0, state_map}(Game2, AEAD_Reduction.R)
+         /\ Game2.psk_map{1} = AEAD_Oracles_common.key_map{2}
+         /\ (forall a b m1, Game2.dec_map{1}.[msg1_data a b, m1] = AEAD_Oracles_1.dec_map{2}.[(a, b), msg1_data a b, m1])
+         /\ (forall a b m1 m2, Game2.dec_map{1}.[msg2_data a b m1, m2] = AEAD_Oracles_1.dec_map{2}.[(a, b), msg2_data a b m1, m2])
+         /\ (forall a b m1 m2 m3, Game2.dec_map{1}.[msg3_data a b m1 m2, m3] = AEAD_Oracles_1.dec_map{2}.[(a, b), msg3_data a b m1 m2, m3])
   ) Game2_inv_send_fin _ => //.
   proc; inline.
-  sp; wp ^if ^if; if=> //.
+  sp; wp ^if ^if; if => //.
   sp; match = => //.
   + smt().
-  move=> st m1 m2.
+  move => st m1 m2.
   rcondt {2} 6.
   + auto=> />.
     smt(get_setE).
-  by sp; match =; auto.
+  by sp; match =; auto; smt(get_setE).
 
 - conseq (: ={res}
-       /\ ={psk_map}(Game2, GAEADb)
-       /\ ={b0, state_map}(Game2, Red_AEAD.WAKE_O)
-       /\ Game2.dec_map{1} = GAEAD1.ctxts{2}
+         /\ ={b0, state_map}(Game2, AEAD_Reduction.R)
+         /\ Game2.psk_map{1} = AEAD_Oracles_common.key_map{2}
+         /\ (forall a b m1, Game2.dec_map{1}.[msg1_data a b, m1] = AEAD_Oracles_1.dec_map{2}.[(a, b), msg1_data a b, m1])
+         /\ (forall a b m1 m2, Game2.dec_map{1}.[msg2_data a b m1, m2] = AEAD_Oracles_1.dec_map{2}.[(a, b), msg2_data a b m1, m2])
+         /\ (forall a b m1 m2 m3, Game2.dec_map{1}.[msg3_data a b m1 m2, m3] = AEAD_Oracles_1.dec_map{2}.[(a, b), msg3_data a b m1 m2, m3])
   ) Game2_inv_reveal _ => //.
-  by sim.
+  by sim />.
 
 - conseq (: ={res}
-       /\ ={psk_map}(Game2, GAEADb)
-       /\ ={b0, state_map}(Game2, Red_AEAD.WAKE_O)
-       /\ Game2.dec_map{1} = GAEAD1.ctxts{2}
+         /\ ={b0, state_map}(Game2, AEAD_Reduction.R)
+         /\ Game2.psk_map{1} = AEAD_Oracles_common.key_map{2}
+         /\ (forall a b m1, Game2.dec_map{1}.[msg1_data a b, m1] = AEAD_Oracles_1.dec_map{2}.[(a, b), msg1_data a b, m1])
+         /\ (forall a b m1 m2, Game2.dec_map{1}.[msg2_data a b m1, m2] = AEAD_Oracles_1.dec_map{2}.[(a, b), msg2_data a b m1, m2])
+         /\ (forall a b m1 m2 m3, Game2.dec_map{1}.[msg3_data a b m1 m2, m3] = AEAD_Oracles_1.dec_map{2}.[(a, b), msg3_data a b m1 m2, m3])
   ) Game2_inv_test _ => //.
-  by sim.
+  by sim />.
  
 auto => />.
 smt(emptyE).
 qed.
 
 (* ------------------------------------------------------------------------------------------ *)
-(* Step 2a: Remove collisions of all produced ciphertexts. *)
+(* Hop 4: Game 2 to Game 3 - Remove collisions of all produced ciphertexts. *)
 
-lemma Step2 bit &m: `| Pr[E_GAKE(Game2, A).run(bit) @ &m : res] - Pr[E_GAKE(Game3, A).run(bit) @ &m : res] | <= Pr[E_GAKE(Game2, A).run(bit) @ &m : Game2.bad].
+lemma Hop4 bit &m: `| Pr[AKE_Game(Game2, A).run(bit) @ &m : res] - Pr[AKE_Game(Game3, A).run(bit) @ &m : res] | <= Pr[AKE_Game(Game2, A).run(bit) @ &m : Game2.bad].
 proof.
 rewrite StdOrder.RealOrder.distrC.
 byequiv (: _ ==> _) : Game3.bad => //; first last.
-+ move=> &1 &2.
++ move => &1 &2.
   by case: (Game2.bad{2}).
 symmetry; proc; inline*.
 call (: Game3.bad, ={b0, bad, psk_map, state_map, dec_map}(Game2, Game3), ={bad}(Game2, Game3)) => //.
 + exact A_ll.
 
 + by proc; inline*; auto; if; auto.
-+ move=> &2 ->.
-  proc; sp; if; auto=> />.
++ move => &2 ->.
+  proc; sp; if; auto => />.
   by rewrite dpskey_ll.
-+ move=> &1.
++ move => &1.
   proc; sp; if; auto.
   by rewrite dpskey_ll.
 
 + proc.
-  sp; wp; if=> //.
+  sp; wp; if => //.
   seq 1 1: (#pre /\ ={ca}); 1: by auto.
   sp 1 1.
-  by if{2}; auto=> />.
-+ move=> &2 ->.
-  proc; sp; if=> //; auto.
+  by if{2}; auto => />.
++ move => &2 ->.
+  proc; sp; if => //; auto.
   by rewrite dnonce_ll dctxt_ll.
-+ move=> &1.
-  proc; sp; wp; if=> //.
-  rcondf ^if; auto=> />.
++ move => &1.
+  proc; sp; wp; if => //.
+  rcondf ^if; auto => />.
   by rewrite dctxt_ll.
 
 + proc.
-  sp; wp; if=> //.
+  sp; wp; if => //.
   match = => //.
   + by auto.
-  move=> na.
+  move => na.
   seq 1 1: (#pre /\ ={cb}); 1: by auto.
   sp 0 1.
-  by if{2}; auto=> />.
-+ move=> &2 ->.
-  proc; sp; wp; if=> //; match =; auto.
+  by if{2}; auto => />.
++ move => &2 ->.
+  proc; sp; wp; if => //; match =; auto.
   by rewrite dnonce_ll dctxt_ll.
-+ move=> &1.
-  proc; sp; wp; if=> //; match =; auto.
-  rcondf ^if; auto=> />.
++ move => &1.
+  proc; sp; wp; if => //; match =; auto.
+  rcondf ^if; auto => />.
   by rewrite dctxt_ll.
 
 + proc.
-  sp; wp; if=> //.
+  sp; wp; if => //.
   sp; match = => //.
   - smt().
   move => s m1.
   sp; match = => //.
   + by auto.
-  move=> nb.
-  seq 1 1: (#pre /\ ={caf}); 1: by auto.
+  move => nb.
+  seq 1 1: (#pre /\ ={cok}); 1: by auto.
   sp 0 1.
   by if{2}; auto=> />.
-+ move=> &2 ->.
-  proc; sp; wp; if=> //; sp; match =; auto; sp; match =; auto.
++ move => &2 ->.
+  proc; sp; wp; if => //; sp; match =; auto; sp; match =; auto.
   by rewrite dnonce_ll dctxt_ll.
-+ move=> &1.
-  proc; sp; wp; if=> //; sp; match =; auto; sp; match =; auto.
-  rcondf ^if; auto=> />.
++ move => &1.
+  proc; sp; wp; if => //; sp; match =; auto; sp; match =; auto.
+  rcondf ^if; auto => />.
   by rewrite dctxt_ll.
 
 + proc.
   sp; wp ^if ^if; if=> //.
   sp; match =; auto; smt().
-+ move=> &2 ->.
-  proc; sp; wp ^if; if=> //; sp; match =; auto; smt().
-+ move=> &1.
-  proc; sp; wp ^if; if=> //; sp; match =; auto; smt().
++ move => &2 ->.
+  proc; sp; wp ^if; if => //; sp; match =; auto; smt().
++ move => &1.
+  proc; sp; wp ^if; if => //; sp; match =; auto; smt().
 
 + proc.
-  sp; wp ^if ^if ;if=> //.
+  sp; wp ^if ^if ;if => //.
   sp; match =; auto; smt().
-+ move=> &2 ->.
-  proc; sp; wp ^if; if=> //; sp; match =; auto; smt().
-+ move=> &1.
-  proc; sp; wp ^if; if=> //; sp; match =; auto; smt().
-
++ move => &2 ->.
+  proc; sp; wp ^if; if => //; sp; match =; auto; smt().
++ move => &1.
+  proc; sp; wp ^if; if => //; sp; match =; auto; smt().
 
 + proc.
-  sp; wp ^if ^if; if=> //.
+  sp; wp ^if ^if; if => //.
   sp; match =; auto.
   + smt().
   sp; if => //; if => //; auto => /#.
 + move=> &2 ->.
-  proc; sp; wp ^if; if=> //; sp; match =; auto.
+  proc; sp; wp ^if; if => //; sp; match =; auto.
   sp; if => //; if => //.
   + auto => /#.
   auto => />.
   by rewrite dskey_ll.
-+ move=> &1.
-  proc; sp; wp ^if; if=> //; sp; match =; auto.
++ move => &1.
+  proc; sp; wp ^if; if => //; sp; match =; auto.
   sp; if => //; if => //.
   + auto => /#.
   auto => />.
   by rewrite dskey_ll.
-auto=> />.
-move=> rl rr al bl dl pl sl ar br dr pr sr.
+auto => />.
+move => rl rr al bl dl pl sl ar br dr pr sr.
 by case : (!br) => />.
 qed.
 
 (* ------------------------------------------------------------------------------------------ *)
 (* Step 2b: Bound the bad event. *)
 
-lemma Step2b bit &m: Pr[E_GAKE(Game2, A).run(bit) @ &m : Game2.bad] <= ((q_m1 + q_m2 + q_m3) ^ 2)%r * mu1 dctxt (mode dctxt).
+lemma Hop4_bound bit &m: Pr[AKE_Game(Game2, A).run(bit) @ &m : Game2.bad] <= ((q_m1 + q_m2 + q_m3) ^ 2)%r * mu1 dctxt (mode dctxt).
 proof.
 case (bit) => real_ideal.
 
 (* Proof for the ideal side *)
-apply (StdOrder.RealOrder.ler_trans Pr[BD.Exp(BD.Sample, Red_Coll_ideal(A)).main() @ &m : !uniq BD.Sample.l]); first last.
-+ apply (BD.pr_collision_q2 (Red_Coll_ideal(A))).
+apply (StdOrder.RealOrder.ler_trans Pr[BD.Exp(BD.Sample, Collision_Reduction_1(A)).main() @ &m : !uniq BD.Sample.l]); first last.
++ apply (BD.pr_collision_q2 (Collision_Reduction_1(A))).
   + move => S S_ll.
     islossless.
-    apply (A_ll (Counter(Red_Coll_O_WAKE(S)))); islossless.
+    apply (A_ll (Counter(Collision_Reduction_Oracles(S)))); islossless.
     + by match; auto; islossless.
     + match; auto.
       by sp; match; auto; islossless.
@@ -802,63 +862,63 @@ apply (StdOrder.RealOrder.ler_trans Pr[BD.Exp(BD.Sample, Red_Coll_ideal(A)).main
   sp.
   conseq (: _ ==> size BD.Sample.l <= Counter.cm1 + Counter.cm2 + Counter.cm3) (: Counter.cm1 = 0 /\ Counter.cm2 = 0 /\ Counter.cm3 = 0 ==> Counter.cm1 <= q_m1 /\ Counter.cm2 <= q_m2 /\ Counter.cm3 <= q_m3)=> //.
   + smt().
-  + by call (A_bounded_qs (Red_Coll_O_WAKE(BD.Sample))).
+  + by call (A_bounded_qs (Collision_Reduction_Oracles(BD.Sample))).
   call (: size BD.Sample.l <= Counter.cm1 + Counter.cm2 + Counter.cm3) => //.
-  + proc; inline*; if; auto.
-  + proc; inline*; sp; if => //; auto => /#.
+  + by proc; inline*; if; auto.
+  + by proc; inline*; sp; if => //; auto => /#.
   + proc; inline*.
     sp; if => //.
-    + case ((Red_Coll_O_WAKE.dec_map.[(a, b), msg1_data a b, ca]) = None).
+    + case ((Collision_Reduction_Oracles.dec_map.[msg1_data a b, ca]) = None).
       + match None ^match => //.
-        auto => /#.
-      match Some ^match => //; auto => /#.
-    auto => /#.
+        by auto => /#.
+      by match Some ^match => //; auto => /#.
+    by auto => /#.
   + proc; inline*.
     sp; if => //.
-    + sp; match; 2,3,4,5: auto => /#.
-      case ((Red_Coll_O_WAKE.dec_map.[(a, s.`1), msg2_data a s.`1 s.`4, m2]) = None).
+    + sp; match; ~1: by auto => /#.
+      case ((Collision_Reduction_Oracles.dec_map.[msg2_data m1.`1 si.`1 m1.`2, m2]) = None).
       + match None ^match => //.
         + by auto => />.
         by auto => /#.
       by match Some ^match => //; auto => /#.
-    auto => /#.
-  + proc; inline*; auto => /#.
-  + proc; inline*; auto => /#.
+    by auto => /#.
+  + by proc; inline*; auto => /#.
+  + by proc; inline*; auto => /#.
   + proc; inline*; sp; if => //; sp; match => //.
-    sp; if => //; sp; if => //; auto => /#.
-  auto=> /#.
+    by sp; if => //; sp; if => //; auto => /#.
+  by auto=> /#.
 
 byequiv => //.
 proc; inline.
 call (:
- ={b0, state_map, psk_map, bad, dec_map}(Game2, Red_Coll_O_WAKE(BD.Sample))
+ ={b0, state_map, psk_map, bad, dec_map}(Game2, Collision_Reduction_Oracles(BD.Sample))
  /\ (Game2.bad{1} => !uniq BD.Sample.l{2})
- /\ (forall c, (exists pk ad, (pk, ad, c) \in Red_Coll_O_WAKE.dec_map) => c \in BD.Sample.l){2}
+ /\ (forall c, (exists ad, (ad, c) \in Collision_Reduction_Oracles.dec_map) => c \in BD.Sample.l){2}
 ) => //.
 
 + by sim />.
 
 + proc; inline.
-  sp; if=> //; auto=> />.
+  sp; if => //; auto=> />.
   smt(mem_set).
 
 + proc; inline.
-  sp; if=> //; 2: by auto=> />.
+  sp; if => //; 2: by auto => />.
   sp; match = => //.
   + by auto => />.
-  move=> na.
-  auto=> />.
+  move => na.
+  auto => />.
   smt(mem_set).
 
 + proc; inline.
-  sp; if=> //; 2: by auto=> />.
-  sp; match =; auto=> />.
+  sp; if=> //; 2: by auto => />.
+  sp; match =; auto => />.
   + smt().
   + smt().
   sp; match = => //.
-  + by auto=> /#.
-  move=> nb.
-  auto=> />.
+  + by auto => /#.
+  move => nb.
+  auto => />.
   smt(mem_set).
 
 + by sim />.
@@ -867,15 +927,15 @@ call (:
 
 by sim />.
 
-auto=> />.
+auto => />.
 smt(emptyE).
 
 (* Proof for the real side *)
-apply (StdOrder.RealOrder.ler_trans Pr[BD.Exp(BD.Sample, Red_Coll_real(A)).main() @ &m : !uniq BD.Sample.l]); first last.
-+ apply (BD.pr_collision_q2 (Red_Coll_real(A))).
+apply (StdOrder.RealOrder.ler_trans Pr[BD.Exp(BD.Sample, Collision_Reduction_0(A)).main() @ &m : !uniq BD.Sample.l]); first last.
++ apply (BD.pr_collision_q2 (Collision_Reduction_0(A))).
   + move => S S_ll.
     islossless.
-    apply (A_ll (Counter(Red_Coll_O_WAKE(S)))); islossless.
+    apply (A_ll (Counter(Collision_Reduction_Oracles(S)))); islossless.
     + by match; auto; islossless.
     + match; auto.
       by sp; match; auto; islossless.
@@ -885,65 +945,65 @@ apply (StdOrder.RealOrder.ler_trans Pr[BD.Exp(BD.Sample, Red_Coll_real(A)).main(
     by match; islossless.
   proc; inline.
   sp.
-  conseq (: _ ==> size BD.Sample.l <= Counter.cm1 + Counter.cm2 + Counter.cm3) (: Counter.cm1 = 0 /\ Counter.cm2 = 0 /\ Counter.cm3 = 0 ==> Counter.cm1 <= q_m1 /\ Counter.cm2 <= q_m2 /\ Counter.cm3 <= q_m3)=> //.
+  conseq (: _ ==> size BD.Sample.l <= Counter.cm1 + Counter.cm2 + Counter.cm3) (: Counter.cm1 = 0 /\ Counter.cm2 = 0 /\ Counter.cm3 = 0 ==> Counter.cm1 <= q_m1 /\ Counter.cm2 <= q_m2 /\ Counter.cm3 <= q_m3) => //.
   + smt().
-  + by call (A_bounded_qs (Red_Coll_O_WAKE(BD.Sample))).
+  + by call (A_bounded_qs (Collision_Reduction_Oracles(BD.Sample))).
   call (: size BD.Sample.l <= Counter.cm1 + Counter.cm2 + Counter.cm3) => //.
-  + proc; inline*; if; auto.
-  + proc; inline*; sp; if => //; auto => /#.
+  + by proc; inline*; if; auto.
+  + by proc; inline*; sp; if => //; auto => /#.
   + proc; inline*.
     sp; if => //.
-    + case ((Red_Coll_O_WAKE.dec_map.[(a, b), msg1_data a b, ca]) = None).
+    + case ((Collision_Reduction_Oracles.dec_map.[msg1_data a b, ca]) = None).
       + match None ^match => //.
         auto => /#.
-      match Some ^match => //; auto => /#.
-    auto => /#.
+      by match Some ^match => //; auto => /#.
+    by auto => /#.
   + proc; inline*.
     sp; if => //.
-    + sp; match; 2,3,4,5: auto => /#.
-      case ((Red_Coll_O_WAKE.dec_map.[(a, s.`1), msg2_data a s.`1 s.`4, m2]) = None).
+    + sp; match; ~1: by auto => /#.
+      case ((Collision_Reduction_Oracles.dec_map.[msg2_data m1.`1 si.`1 m1.`2, m2]) = None).
       + match None ^match => //.
         + by auto => />.
         by auto => /#.
       by match Some ^match => //; auto => /#.
-    auto => /#.
-  + proc; inline*; auto => /#.
-  + proc; inline*; auto => /#.
+    by auto => /#.
+  + by proc; inline*; auto => /#.
+  + by proc; inline*; auto => /#.
   + proc; inline*; sp; if => //; sp; match => //.
-    sp; if => //; sp; if => //; auto => /#.
-  auto=> /#.
+    by sp; if => //; sp; if => //; auto => /#.
+  by auto => /#.
 
 byequiv => //.
 proc; inline.
 call (:
- ={b0, state_map, psk_map, bad, dec_map}(Game2, Red_Coll_O_WAKE(BD.Sample))
+ ={b0, state_map, psk_map, bad, dec_map}(Game2, Collision_Reduction_Oracles(BD.Sample))
  /\ (Game2.bad{1} => !uniq BD.Sample.l{2})
- /\ (forall c, (exists pk ad, (pk, ad, c) \in Red_Coll_O_WAKE.dec_map) => c \in BD.Sample.l){2}
+ /\ (forall c, (exists ad, (ad, c) \in Collision_Reduction_Oracles.dec_map) => c \in BD.Sample.l){2}
 ) => //.
 
 + by sim />.
 
 + proc; inline.
-  sp; if=> //; auto=> />.
+  sp; if => //; auto=> />.
   smt(mem_set).
 
 + proc; inline.
-  sp; if=> //; 2: by auto=> />.
+  sp; if => //; 2: by auto => />.
   sp; match = => //.
   + by auto => />.
-  move=> na.
-  auto=> />.
+  move => na.
+  auto => />.
   smt(mem_set).
 
 + proc; inline.
-  sp; if=> //; 2: by auto=> />.
-  sp; match =; auto=> />.
+  sp; if=> //; 2: by auto => />.
+  sp; match =; auto => />.
   + smt().
   + smt().
   sp; match = => //.
-  + by auto=> /#.
-  move=> nb.
-  auto=> />.
+  + by auto => /#.
+  move => nb.
+  auto => />.
   smt(mem_set).
 
 + by sim />.
@@ -957,99 +1017,89 @@ smt(emptyE).
 qed.
 
 (* ------------------------------------------------------------------------------------------ *)
-(* Step 3: No longer store nonces in the state, just retrieve from the dec_map. *)
+(* Hop 5: Game 3 to Game 3a - Retrieve nonces from the dec_map not session state. *)
 
-local op clear_nonces (s : instance_state) =
+local op clean2 (s : session_state) =
 match s with
 | IPending st m1 =>
-  let (id, psk, na, ca) = st in IPending (id, psk, witness, ca) m1
+  let (id, psk, na, ca) = st in IPending (id, witness, witness, witness) m1
 | RPending st m1 m2 =>
-  let (id, psk, na, nb, ca, cb) = st in RPending (id, psk, witness, witness, ca, cb) m1 m2
+  let (id, psk, na, nb, ca, cb) = st in RPending (witness, witness, witness, witness, witness, witness) m1 m2
 | Accepted _ _ => s
 | Observed _ _ => s
 | Aborted   => s
 end.
 
-local lemma eq_partners_nonces tr r sml smr:
-  (forall h, omap (fun (v: role * instance_state) => let (r, s) = v in (r, clear_nonces s)) sml.[h] = smr.[h]) =>
-get_partners tr r sml = get_partners tr r smr.
+local lemma clean2_fresh h sml smr:
+  (forall h, omap (fun (v: _ * _) => let (r, s) = v in (r, clean2 s)) sml.[h] = smr.[h]) =>
+  fresh h sml <=> fresh h smr.
 proof.
-move=> eqsm.
-rewrite /get_partners.
-congr.
-apply fmap_eqP => h'.
-rewrite !filterE -(eqsm h') /=.
-case: (sml.[h'])=> //=.
-by move=> [r' []] // [] /= /#.
+move=> eq_sm.
+rewrite /fresh.
+have eq_ps : partners h sml = partners h smr.
++ rewrite /partners.
+  congr.
+  apply fmap_eqP => h'.
+  rewrite !filterE -(eq_sm h') /=.
+  by case: (sml.[h']); smt().
+rewrite /observed_partners eq_ps.
+do! congr.
+rewrite fun_ext => h'.
+rewrite -(eq_sm h') //=.
+case: (sml.[h'])=> //.
+by move => [r' []] // [].
 qed.
 
-local lemma eq_obs_partners_nonces h sml smr:
-  (forall h, omap (fun (v: role * instance_state) => let (r, s) = v in (r, clear_nonces s)) sml.[h] = smr.[h]) =>
-get_observed_partners h sml = get_observed_partners h smr.
-proof.
-move=> eqsm.
-rewrite /get_observed_partners.
-congr.
-+ rewrite fun_ext => bj.
-  rewrite -(eqsm bj) //=.
-  case: (sml.[bj])=> //.
-  by move=> [r' []] // [].
-rewrite -(eq_partners_nonces _ _ sml smr eqsm).
-rewrite -(eqsm h) /s /r //=.
-case: (sml.[h])=> //.
-by move=> [r' []] // [].
-qed.
-
-lemma Step3 bit &m: Pr[E_GAKE(Game3, A).run(bit) @ &m : res] = Pr[E_GAKE(Game4, A).run(bit) @ &m :res].
+lemma Hop5 bit &m: Pr[AKE_Game(Game3, A).run(bit) @ &m : res] = Pr[AKE_Game(Game3a, A).run(bit) @ &m :res].
 proof.
 byequiv (: ={glob A, arg} ==> _) => //.
 proc; inline*.
-call(: ={b0, psk_map, bad, dec_map}(Game3, Game4)
-    /\ (forall h, omap (fun v => let (r, s) = v in (r, clear_nonces s)) Game3.state_map.[h]{1} = Game4.state_map.[h]{2})
+call(: ={b0, psk_map, bad, dec_map}(Game3, Game3a)
+    /\ (forall h, omap (fun v => let (r, s) = v in (r, clean2 s)) Game3.state_map.[h]{1} = Game3a.state_map.[h]{2})
     /\ (forall a i, Game3_inv Game3.state_map Game3.dec_map a i){1}
 ).
 
 - conseq (: ={res}
-    /\ ={b0, psk_map, bad, dec_map}(Game3, Game4)
-    /\ (forall h, omap (fun v => let (r, s) = v in (r, clear_nonces s)) Game3.state_map.[h]{1} = Game4.state_map.[h]{2})
+    /\ ={b0, psk_map, bad, dec_map}(Game3, Game3a)
+    /\ (forall h, omap (fun v => let (r, s) = v in (r, clean2 s)) Game3.state_map.[h]{1} = Game3a.state_map.[h]{2})
   ) Game3_inv_gen_pskey _ => //.
   proc.
   by if; auto.
 
 - conseq (: ={res}
-    /\ ={b0, psk_map, bad, dec_map}(Game3, Game4)
-    /\ (forall h, omap (fun v => let (r, s) = v in (r, clear_nonces s)) Game3.state_map.[h]{1} = Game4.state_map.[h]{2})
+    /\ ={b0, psk_map, bad, dec_map}(Game3, Game3a)
+    /\ (forall h, omap (fun v => let (r, s) = v in (r, clean2 s)) Game3.state_map.[h]{1} = Game3a.state_map.[h]{2})
   ) Game3_inv_send_msg1 _ => //.
   proc; inline*.
-  sp; wp; if=> //.
+  sp; wp; if => //.
   + smt().
   seq 1 1 : (#pre /\ ={ca}); 1: by auto.
-  sp; if=> //.
+  sp; if => //.
   sp; seq 1 1 : (#pre /\ ={na}); 1: by auto=> />.
-  auto=> />.
+  auto => />.
   smt(get_setE).
 
 - conseq (: ={res}
-    /\ ={b0, psk_map, bad, dec_map}(Game3, Game4)
-    /\ (forall h, omap (fun v => let (r, s) = v in (r, clear_nonces s)) Game3.state_map.[h]{1} = Game4.state_map.[h]{2})
+    /\ ={b0, psk_map, bad, dec_map}(Game3, Game3a)
+    /\ (forall h, omap (fun v => let (r, s) = v in (r, clean2 s)) Game3.state_map.[h]{1} = Game3a.state_map.[h]{2})
   ) Game3_inv_send_msg2 _ => //.
   proc; inline*.
-  sp; wp; if=> //.
+  sp; wp; if => //.
   + smt().
   match = => //.
   + by auto; smt(get_setE).
-  move=> na.
+  move => na.
   seq 1 1 : (#pre /\ ={cb}); 1: by auto.
-  sp; if=> //.
-  auto=> />.
+  sp; if => //.
+  auto => />.
   smt(get_setE).
 
 - conseq (: ={res}
-    /\ ={b0, psk_map, bad, dec_map}(Game3, Game4)
-    /\ (forall h, omap (fun v => let (r, s) = v in (r, clear_nonces s)) Game3.state_map.[h]{1} = Game4.state_map.[h]{2})
+    /\ ={b0, psk_map, bad, dec_map}(Game3, Game3a)
+    /\ (forall h, omap (fun v => let (r, s) = v in (r, clean2 s)) Game3.state_map.[h]{1} = Game3a.state_map.[h]{2})
   ) Game3_inv_send_msg3 _ => //.
   proc; inline*.
-  sp; wp; if=> //.
+  sp; wp; if => //.
   + smt().
   sp; match; 1..5: (
     move=> &1 &2 /> + + /(_ (a, i){2});
@@ -1057,23 +1107,23 @@ call(: ={b0, psk_map, bad, dec_map}(Game3, Game4)
     case: (Game3.state_map{1}.[(a, i)]{2})=> />;
     move=> + H;
     by rewrite -H => /#
-  ); 2..5: by auto.
-  move=> sl m1l sr m1r.
+  ); ~1: by auto.
+  move => sl m1l sr m1r.
   sp; match = => //.
-  + auto=> /> /#.
+  + auto => /> /#.
   + by auto => />; smt(get_setE).
-  move=> nb.
-  seq 1 1 : (#pre /\ ={caf}); 1: by auto.
-  sp; if=> //.
-  auto=> />.
-  smt(get_setE).
+  move => nb.
+  seq 1 1 : (#pre /\ ={cok}); 1: by auto.
+  sp; if => //.
+  auto => /> *.
+  by do split; smt(get_setE).
 
 - conseq (: ={res}
-    /\ ={b0, psk_map, bad, dec_map}(Game3, Game4)
-    /\ (forall h, omap (fun v => let (r, s) = v in (r, clear_nonces s)) Game3.state_map.[h]{1} = Game4.state_map.[h]{2})
+    /\ ={b0, psk_map, bad, dec_map}(Game3, Game3a)
+    /\ (forall h, omap (fun v => let (r, s) = v in (r, clean2 s)) Game3.state_map.[h]{1} = Game3a.state_map.[h]{2})
   ) Game3_inv_send_fin _ => //.
   proc; inline*.
-  sp; wp ^if ^if; if=> //.
+  sp; wp ^if ^if; if => //.
   + smt().
   sp; match; 1..5: (
     move=> &1 &2 /> + + /(_ (b, j){2});
@@ -1082,455 +1132,527 @@ call(: ={b0, psk_map, bad, dec_map}(Game3, Game4)
     move=> + H;
     by rewrite -H => /#
   ); 1,3..5: by auto.
-  move=> sl m1l m2l sr m1r m2r.
+  move => sl m1l m2l sr m1r m2r.
   sp; match = => //.
-  + move=> /> /#.
+  + move => /> /#.
   + by auto => />; smt(get_setE).
-  move=> nok.
-  auto=> />.
+  move => nok.
+  auto => />.
   smt(get_setE).
 
 - conseq (: ={res}
-    /\ ={b0, psk_map, bad, dec_map}(Game3, Game4)
-    /\ (forall h, omap (fun v => let (r, s) = v in (r, clear_nonces s)) Game3.state_map.[h]{1} = Game4.state_map.[h]{2})
+    /\ ={b0, psk_map, bad, dec_map}(Game3, Game3a)
+    /\ (forall h, omap (fun v => let (r, s) = v in (r, clean2 s)) Game3.state_map.[h]{1} = Game3a.state_map.[h]{2})
   ) Game3_inv_reveal _ => //.
   proc; inline.
-  sp; wp ^if ^if; if=> //.
+  sp; wp ^if ^if; if => //.
   + smt().
   sp; match; 1..5:(
-    move=> &1 &2 /> + + /(_ (a, i){2});
+    move => &1 &2 /> + + /(_ h{2});
     rewrite domE;
-    case: (Game3.state_map{1}.[(a, i)]{2})=> />;
-    move=> + H;
+    case: (Game3.state_map{1}.[h{2}]) => />;
+    move => + H;
     by rewrite -H => /#
-  ); 1,2,4,5: by auto.
-  move=> tr k tr' k'.
-  sp ^if & -1 ^if & -1; if=> //.
-  + move => &1 &2 [] /> *.
-    by rewrite (eq_obs_partners_nonces (a, i){2} Game3.state_map{1} Game4.state_map{2}) => //.
-  auto=> /> &1 &2 + + eqsm invl a_in _.
-  rewrite -(eqsm (a, i){2}).
+  ); ~3: by auto.
+  move=> t k t' k'.
+  sp ^if & -1 ^if & -1; if => //.
+  + move => &1 &2 [] |> *.
+    by rewrite (clean2_fresh h{2} Game3.state_map{1} Game3a.state_map{2}).
+  auto => /> &1 &2 + + eqsm invl a_in _.
+  rewrite -(eqsm h{2}).
   move => *.
   split. smt().
-  move => h.
-  case (h = (a, i){2}) => [|hneq].
+  move => h'.
+  case (h' = h{2}) => [|hneq].
   smt(get_set_sameE).
   do rewrite get_set_neqE => //.
   by rewrite eqsm.
 
 - conseq (: ={res}
-    /\ ={b0, psk_map, bad, dec_map}(Game3, Game4)
-    /\ (forall h, omap (fun v => let (r, s) = v in (r, clear_nonces s)) Game3.state_map.[h]{1} = Game4.state_map.[h]{2})
+    /\ ={b0, psk_map, bad, dec_map}(Game3, Game3a)
+    /\ (forall h, omap (fun v => let (r, s) = v in (r, clean2 s)) Game3.state_map.[h]{1} = Game3a.state_map.[h]{2})
   ) Game3_inv_test _ => //.
   proc; inline.
   sp; wp ^if ^if; if=> //.
   + smt().
   sp; match; 1..5:(
-    move=> &1 &2 /> + + /(_ (a, i){2});
+    move => &1 &2 /> + + /(_ h{2});
     rewrite domE;
-    case: (Game3.state_map{1}.[(a, i)]{2})=> />;
-    move=> + H;
+    case: (Game3.state_map{1}.[h]{2}) => />;
+    move => + H;
     by rewrite -H => /#
-  ); 1,2,4,5: by auto.
-  move=> tr k tr' k'.
-  sp ^if & -1 ^if & -1; if=> //.
-  + move => &1 &2 [] /> *.
-    by rewrite (eq_obs_partners_nonces (a, i){2} Game3.state_map{1} Game4.state_map{2}) => //.
+  ); ~3: by auto.
+  move=> t k t' k'.
+  sp ^if & -1 ^if & -1; if => //.
+  + move => &1 &2 [] |> *.
+    by rewrite (clean2_fresh h{2} Game3.state_map{1} Game3a.state_map{2}).
   if => //.
   + auto=> /> &1 &2 + + eqsm invl a_in _.
-    rewrite -(eqsm (a, i){2}).
+    rewrite -(eqsm h{2}).
     move => *.
     split. smt().
-    move => h.
-    case (h = (a, i){2}) => [|hneq].
+    move => h'.
+    case (h' = h{2}) => [|hneq].
     smt(get_set_sameE).
     do rewrite get_set_neqE => //.
     by rewrite eqsm.
-  auto=> /> &1 &2 + + eqsm invli invlr a_in _ ideal sk _.
-  rewrite -(eqsm (a, i){2}).
-  move => stm1 stm2 h.
-  case (h = (a, i){2}) => [|hneq].
-  + smt(get_set_sameE).
-  do rewrite get_set_neqE => //.
-  by rewrite eqsm.
+  auto=> |> &1 &2 + + eqsm invli invlr _ ideal sk _.
+  move => ? ? h'.
+  rewrite !get_setE.
+  rewrite -!(eqsm h').
+  by case (h' = h{2}) => //#.
 
 auto=> />.
 smt(emptyE).
 qed.
 
 (* ------------------------------------------------------------------------------------------ *)
-(* Step 4: Delay the sampling of na and nb until msg3, sampling them together. *)
+(* Hop 6: Game 3a to Game 3b - Store nonces separately to logging decryptions *)
+lemma Hop6 bit &m: Pr[AKE_Game(Game3a, A).run(bit) @ &m : res] = Pr[AKE_Game(Game3b, A).run(bit) @ &m : res].
+proof.
+byequiv => //.
+proc; inline.
+call (: ={b0, state_map, psk_map, bad}(Game3a, Game3b)
+      /\ (forall a b m1, Game3a.dec_map.[msg1_data a b, m1]{1} = Game3b.nonce_map.[msg1_data a b, m1]{2})
+      /\ (forall a b m1 m2, Game3a.dec_map.[msg2_data a b m1, m2]{1} = Game3b.nonce_map.[msg2_data a b m1, m2]{2})
+      /\ (forall h, h \in Game3a.dec_map{1} <=> h \in Game3b.dec_map{2})
+); try by sim />.
 
-local clone import DProd.ProdSampling with
-  type t1 <- nonce,
-  type t2 <- nonce
-proof *.
++ proc; inline.
+  sp; if => //.
+  seq 1 1 : (#pre /\ ={ca}); 1: by auto.
+  sp; if.
+  + smt().
+  + sp; seq 1 1 : (#pre /\ ={na}); 1: by auto=> />.
+    auto => />.
+    smt(get_setE mem_set).
+  by auto => /#.
 
-lemma Step4 bit &m: Pr[E_GAKE(Game4, A).run(bit) @ &m : res] = Pr[E_GAKE(Game4', A).run(bit) @ &m : res].
++ proc; inline.
+  sp; if => //.
+  match; 1,2: smt().
+  + by auto; smt().
+  move => *.
+  seq 1 1 : (#pre /\ ={cb}); 1: by auto.
+  sp; if.
+  + smt().
+  + sp; seq 1 1 : (#pre /\ ={nb}); 1: by auto=> />.
+    auto => />.
+    smt(get_setE mem_set).
+  by auto => /#.
+
++ proc; inline.
+  sp; if => //.
+  sp; match = => //.
+  + smt().
+  move => si m1.
+  sp; match; 1,2: smt().
+  + by auto; smt().
+  move => *.
+  seq 1 1 : (#pre /\ ={cok}); 1: by auto.
+  sp; if.
+  + smt().
+  + sp; seq 1 1 : (#pre /\ ={nok}); 1: by auto=> />.
+    auto => />.
+    smt(get_setE).
+  by auto => /#.
+
++ proc; inline.
+  sp; if => //.
+  sp; match = => //.
+  + smt().
+  move => sr m1 m2.
+  sp; match; 1,2: smt().
+  + by auto; smt().
+  move => *.
+  auto => />.
+  smt(get_setE).
+
+by auto.
+qed.
+
+(* ------------------------------------------------------------------------------------------ *)
+(* Hop 7: Game 3b to Game 3c - Delay the sampling of na and nb until first retrieval *)
+
+lemma Hop7 bit &m: Pr[AKE_Game(Game3b, A).run(bit) @ &m : res] = Pr[AKE_Game(Game3c, A).run(bit) @ &m : res].
 byequiv => //.
 proc*.
-transitivity* {1} { r <@ NROc.MainD(Red_ROM(A), NROc.RO).distinguish(b); }.
+transitivity* {1} { r <@ NROc.MainD(Nonce_Delay_Reduction(A), NROc.RO).distinguish(b); }.
 
 + inline*.
   wp.
-  call (: ={b0, state_map, psk_map, bad}(Game4, Red_ROM.WAKE_O)
-       /\ (forall h, h \in Game4.dec_map{1} <=> h \in Red_ROM.WAKE_O.dec_map{2})
-       /\ (forall c ad n, (exists pk, Game4.dec_map{1}.[(pk, ad, c)] = Some n) <=> NROc.RO.m{2}.[(ad, c)] = Some n)
-       /\ (forall a b ca cb, ((a, b), msg2_data a b ca, cb) \in Game4.dec_map => ((a, b), msg1_data a b, ca) \in Game4.dec_map){1}
-       /\ (forall a b ca cb caf, ((a, b), msg3_data a b ca cb, caf) \in Game4.dec_map => ((a, b), msg2_data a b ca, cb) \in Game4.dec_map){1}
+  call (: ={b0, state_map, psk_map, dec_map, bad}(Game3b, Nonce_Delay_Reduction.R)
+       /\ (Game3b.nonce_map{1} = NROc.RO.m{2})
+       /\ (forall a b ca, (msg1_data a b, ca) \in Game3b.dec_map <=> (msg1_data a b, ca) \in Game3b.nonce_map){1}
+       /\ (forall a b ca cb, (msg2_data a b ca, cb) \in Game3b.dec_map <=> (msg2_data a b ca, cb) \in Game3b.nonce_map){1}
+       /\ (forall a b ca cb, (msg2_data a b ca, cb) \in Game3b.dec_map => (msg1_data a b, ca) \in Game3b.dec_map){1}
+       /\ (forall a b ca cb caf, (msg3_data a b ca cb, caf) \in Game3b.dec_map => (msg2_data a b ca, cb) \in Game3b.dec_map){1}
   ) => //.
 
   - by proc; sp; if; auto.
 
   - proc; inline*.
-    sp; wp; if=> //.
+    sp; wp; if => //.
     seq 1 1 : (#pre /\ ={ca}); 1: by auto.
-    sp; if=> //.
+    sp; if => //.
+    rcondt {2} ^if; 1: by auto => /#.
+    auto => />.
+    smt(get_setE).
+
+  - proc; inline*.
+    sp; wp; if => //.
+    match; 1,2: smt().
+    + by auto => />.
+    move=> nal nar.
+    seq 1 1 : (#pre /\ ={cb}); 1: by auto.
+    sp; if => //.
+    rcondt {2} ^if; 1: by auto => /#.
+    auto => />.
+    smt(get_setE).
+
+  - proc; inline*.
+    sp; wp; if => //.
+    sp; match = => //.
     + smt().
-    + rcondt {2} ^if; 1: by auto=> /#.
-      auto=> />.
-      smt(get_setE).
-    by auto=> /#.
+    move => s m1.
+    sp; match; 1: smt().
+    + move => /> *; smt().
+    + by auto => />.
+    move => nbl nbr.
+    seq 1 1 : (#pre /\ ={cok}); 1: by auto.
+    sp; if => //.
+    rcondf {2} ^if.
+    + auto => />.
+      smt(mem_set).
+    rcondf {2} ^if.
+    + auto => />.
+      smt(mem_set).
+    auto => />.
+    smt(get_setE).
 
-   - proc; inline*.
-     sp; wp; if=> //.
-     match; 1,2: smt().
-     + by auto=> />.
-     move=> nal nar.
-     seq 1 1 : (#pre /\ ={cb}); 1: by auto.
-     sp; if=> //.
-     + smt().
-     + rcondt {2} ^if; 1: by auto=> /#.
-       auto=> />.
-       smt(get_setE).
-     by auto=> /#.
+  - proc; inline*.
+    sp; wp ^if ^if; if => //.
+    sp; match = => //.
+    + smt().
+    move => s m1 m2.
+    sp; match; 1,2: smt().
+    + by auto => />.
+    move => nokl nokr.
+    rcondf {2} ^if; 1: by auto => /#.
+    rcondf {2} ^if; 1: by auto => /#.
+    auto => />.
 
-   - proc; inline*.
-     sp; wp; if=> //.
-     sp; match = => //.
-     + smt().
-     move=> s m1.
-     sp; match; 1: smt().
-     + move => /> *; smt().
-     + by auto=> />.
-     move=> nbl nbr.
-     seq 1 1 : (#pre /\ ={caf}); 1: by auto.
-     sp; if=> //.
-     + smt().
-     + rcondt {2} ^if; 1: by auto=> /#.
-       rcondf {2} ^if.
-       + auto=> />.
-         smt(mem_set).
-       rcondf {2} ^if.
-       + auto=> />.
-         smt(mem_set).
-       swap {2} ^r1<$ @ ^ok<-.
-       seq 1 1 : (#pre /\ ok{1} = r1{2}); 1: by auto => />.
-       auto=> />.
-       smt(get_setE).
-    by auto=> /#.
+  - by sim />.
 
-   - proc; inline*.
-     sp; wp ^if ^if; if=> //.
-     sp; match = => //.
-     + smt().
-     move=> s m1 m2.
-     sp; match; 1,2: smt().
-     + by auto=> />.
-     move=> nokl nokr.
-     rcondf {2} ^if; 1: by auto=> /#.
-     rcondf {2} ^if; 1: by auto=> /#.
-     auto=> />.
-     smt(get_setE).
+  - by sim />.
 
-   - by sim />.
+  auto => />.
+  smt(emptyE).
 
-   - by sim />.
-
-   auto=> />.
-   smt(emptyE).
-
-rewrite equiv [{1} 1 (NROc.FullEager.RO_LRO (Red_ROM(A)) _)]; 1: by move=> _; exact dnonce_ll.
+rewrite equiv [{1} 1 (NROc.FullEager.RO_LRO (Nonce_Delay_Reduction(A)) _)]; 1: by move=> _; exact dnonce_ll.
 inline.
 wp; call (:
-  ={b0, state_map, psk_map, bad, dec_map}(Red_ROM.WAKE_O, Game4')
-  /\ NROc.RO.m{1} = Game4'.nonce_map{2}
-
-  (*
-  /\ (forall a b ca, (forall cb caf, (msg3_data a b ca cb, caf) \notin Game5.prfkey_map{2})
-        => (msg1_data a b, ca) \notin NROc.RO.m{1})
-  /\ (forall a b ca cb, (forall caf, (msg3_data a b ca cb, caf) \notin Game5.prfkey_map{2})
-        => (msg2_data a b ca, cb) \notin NROc.RO.m{1})
-  /\ (forall a b ca cb caf, (msg3_data a b ca cb, caf) \in Game5.prfkey_map{2} =>
-         exists na nb, Game5.prfkey_map{2}.[(msg3_data a b ca cb, caf)] = Some (na, nb) /\
-                       NROc.RO.m{1}.[(msg1_data a b, ca)] = Some na /\
-                       NROc.RO.m{1}.[(msg2_data a b ca, cb)] = Some nb)
-  /\ (Game5_inv Game5.state_map Game5.dec_map Game5.prfkey_map){2}
-  *)
+  ={b0, state_map, psk_map, bad, dec_map}(Nonce_Delay_Reduction.R, Game3c)
+  /\ NROc.RO.m{1} = Game3c.nonce_map{2}
 ) => //.
 
 - by sim />.
 
 - proc; inline*.
-  sp; wp; if=> //.
-  auto=> />.
-  smt(mem_set).
+  sp; wp; if => //.
+  by auto => />.
   
 - proc; inline*.
-  sp; wp; if=> //.
-  sp; match =; auto=> />.
-  smt(mem_set).
+  sp; wp; if => //.
+  by sp; match =; auto => />.
 
 - proc; inline*.
-  sp; wp; if=> //.
+  sp; wp; if => //.
   sp; match = => //.
   + smt().
-  move=> s m1.
+  move => si m1.
   sp; match = => //.
   + by auto.
-  move=> nb.
-  seq 1 1 : (#pre /\ ={caf}); 1: by auto.
-  sp; if=> //.
-  rcondt {1} ^if.
-  + auto=> />.
-    admit.
-  rcondt {1} ^if.
-  + auto=> />.
-    admit.
-  auto=> />.
-  smt(mem_set get_setE).
-
-- proc; inline*.
-  sp; wp ^if ^if; if=> //.
-  sp; match = => //.
-  + smt().
-  move=> s m1 m2.
-  sp; match = => //.
-  + by auto.
-  move=> nok.
-  rcondf {1} ^if.
-  + auto=> />.
-    smt().
-  rcondf {1} ^if.
-  + auto=> />.
-    smt().
-  by auto=> />.
-
-- by sim />.
-- by sim />.
+  move => nb.
+  seq 1 1 : (#pre /\ ={cok}); 1: by auto.
+  sp; if => //.
+  swap {1} ^r1<$ @ ^if.
   auto => />.
-  smt(emptyE).
-  qed.
-
-- conseq (: ={res}
-  /\ ={b0, state_map, psk_map, bad, dec_map}(Red_ROM.WAKE_O, Game5)
-  /\ (forall a b ca, (forall cb caf, (msg3_data a b ca cb, caf) \notin Game5.prfkey_map{2})
-        => (msg1_data a b, ca) \notin NROc.RO.m{1})
-  /\ (forall a b ca cb, (forall caf, (msg3_data a b ca cb, caf) \notin Game5.prfkey_map{2})
-        => (msg2_data a b ca, cb) \notin NROc.RO.m{1})
-  /\ (forall a b ca cb caf, (msg3_data a b ca cb, caf) \in Game5.prfkey_map{2} =>
-         exists na nb, Game5.prfkey_map{2}.[(msg3_data a b ca cb, caf)] = Some (na, nb) /\
-                       NROc.RO.m{1}.[(msg1_data a b, ca)] = Some na /\
-                       NROc.RO.m{1}.[(msg2_data a b ca, cb)] = Some nb)
-  ) _ Game5_inv_send_msg1 => //.
-  proc; inline*.
-  sp; wp; if=> //.
-  by auto=> />.
-
-- conseq (: ={res}
-  /\ ={b0, state_map, psk_map, bad, dec_map}(Red_ROM.WAKE_O, Game5)
-  /\ (forall a b ca, (forall cb caf, (msg3_data a b ca cb, caf) \notin Game5.prfkey_map{2})
-        => (msg1_data a b, ca) \notin NROc.RO.m{1})
-  /\ (forall a b ca cb, (forall caf, (msg3_data a b ca cb, caf) \notin Game5.prfkey_map{2})
-        => (msg2_data a b ca, cb) \notin NROc.RO.m{1})
-  /\ (forall a b ca cb caf, (msg3_data a b ca cb, caf) \in Game5.prfkey_map{2} =>
-         exists na nb, Game5.prfkey_map{2}.[(msg3_data a b ca cb, caf)] = Some (na, nb) /\
-                       NROc.RO.m{1}.[(msg1_data a b, ca)] = Some na /\
-                       NROc.RO.m{1}.[(msg2_data a b ca, cb)] = Some nb)
-  ) _ Game5_inv_send_msg2 => //.
-  proc; inline*.
-  sp; wp; if=> //.
-  by sp; match =; auto=> />.
-
-- conseq (: ={res}
-  /\ ={b0, state_map, psk_map, bad, dec_map}(Red_ROM.WAKE_O, Game5)
-  /\ (forall a b ca, (forall cb caf, (msg3_data a b ca cb, caf) \notin Game5.prfkey_map{2})
-        => (msg1_data a b, ca) \notin NROc.RO.m{1})
-  /\ (forall a b ca cb, (forall caf, (msg3_data a b ca cb, caf) \notin Game5.prfkey_map{2})
-        => (msg2_data a b ca, cb) \notin NROc.RO.m{1})
-  /\ (forall a b ca cb caf, (msg3_data a b ca cb, caf) \in Game5.prfkey_map{2} =>
-         exists na nb, Game5.prfkey_map{2}.[(msg3_data a b ca cb, caf)] = Some (na, nb) /\
-                       NROc.RO.m{1}.[(msg1_data a b, ca)] = Some na /\
-                       NROc.RO.m{1}.[(msg2_data a b ca, cb)] = Some nb)
-  ) _ Game5_inv_send_msg3 => //.
-  proc; inline*.
-  sp; wp; if=> //.
-  sp; match = => //.
-  + smt().
-  move=> s m1.
-  sp; match = => //.
-  + by auto.
-  move=> nb.
-  seq 1 1 : (#pre /\ ={caf}); 1: by auto.
-  sp; if=> //.
-  rcondt {1} ^if.
-  + auto=> />.
-    smt().
-  rcondt {1} ^if.
-  + auto=> />.
-    smt(mem_set).
-  outline {2} 3 by {(na, nb') <@ S.sample(dnonce, dnonce);}.
-  wp; rewrite equiv [{2} 3 sample_sample2].
-  inline*.
-  auto=> />.
-  move=> &1 &2 _ dm _ sm _ inv1 inv2 inv3 invr1 invr2 invr3 invr4 /domE/some_oget sms /negb_or [_ cafnin] r _ r1 _.
-  rewrite get_set_sameE //=.
   smt(get_setE).
 
-- conseq (: ={res}
-  /\ ={b0, state_map, psk_map, bad, dec_map}(Red_ROM.WAKE_O, Game5)
-  /\ (forall a b ca, (forall cb caf, (msg3_data a b ca cb, caf) \notin Game5.prfkey_map{2})
-        => (msg1_data a b, ca) \notin NROc.RO.m{1})
-  /\ (forall a b ca cb, (forall caf, (msg3_data a b ca cb, caf) \notin Game5.prfkey_map{2})
-        => (msg2_data a b ca, cb) \notin NROc.RO.m{1})
-  /\ (forall a b ca cb caf, (msg3_data a b ca cb, caf) \in Game5.prfkey_map{2} =>
-         exists na nb, Game5.prfkey_map{2}.[(msg3_data a b ca cb, caf)] = Some (na, nb) /\
-                       NROc.RO.m{1}.[(msg1_data a b, ca)] = Some na /\
-                       NROc.RO.m{1}.[(msg2_data a b ca, cb)] = Some nb)
-  ) _ Game5_inv_send_fin => //.
 - proc; inline*.
-  sp; wp ^if ^if; if=> //.
+  sp; wp ^if ^if; if => //.
   sp; match = => //.
   + smt().
-  move=> s m1 m2.
+  move => sr m1 m2.
   sp; match = => //.
   + by auto.
-  move=> nok.
-  rcondf {1} ^if.
-  + auto=> />.
-    smt().
-  rcondf {1} ^if.
-  + auto=> />.
-    smt().
-  auto=> />.
-  smt().
+  move => nok.
+  swap {1} ^r1<$ @ ^if.
+  auto => />.
+  smt(get_setE).
 
-- conseq (: ={res}
-  /\ ={b0, state_map, psk_map, bad, dec_map}(Red_ROM.WAKE_O, Game5)
-  /\ (forall a b ca, (forall cb caf, (msg3_data a b ca cb, caf) \notin Game5.prfkey_map{2})
-        => (msg1_data a b, ca) \notin NROc.RO.m{1})
-  /\ (forall a b ca cb, (forall caf, (msg3_data a b ca cb, caf) \notin Game5.prfkey_map{2})
-        => (msg2_data a b ca, cb) \notin NROc.RO.m{1})
-  /\ (forall a b ca cb caf, (msg3_data a b ca cb, caf) \in Game5.prfkey_map{2} =>
-         exists na nb, Game5.prfkey_map{2}.[(msg3_data a b ca cb, caf)] = Some (na, nb) /\
-                       NROc.RO.m{1}.[(msg1_data a b, ca)] = Some na /\
-                       NROc.RO.m{1}.[(msg2_data a b ca, cb)] = Some nb)
-  ) _ Game5_inv_reveal => //.
+- by sim />.
+
+- by sim />.
+
+by auto => />.
+qed.
+
+(* ------------------------------------------------------------------------------------------ *)
+(* Hop 8: Game 3c to Game 3d - Remove checks for first sampling retrieval *)
+
+lemma Hop8 bit &m: Pr[AKE_Game(Game3c, A).run(bit) @ &m : res] = Pr[AKE_Game(Game3d, A).run(bit) @ &m : res].
+byequiv => //.
+proc; inline.
+call (: ={b0, state_map, psk_map, dec_map, bad, nonce_map}(Game3c, Game3d)
+      /\ (Game3d_inv Game3d.state_map Game3d.dec_map Game3d.nonce_map){2}
+).
+
++ by sim />.
+
++ conseq (: ={res}
+          /\ ={b0, state_map, psk_map, dec_map, bad, nonce_map}(Game3c, Game3d)
+  ) _ Game3d_inv_send_msg1 => //.
   by sim />.
 
-- conseq (: ={res}
-  /\ ={b0, state_map, psk_map, bad, dec_map}(Red_ROM.WAKE_O, Game5)
-  /\ (forall a b ca, (forall cb caf, (msg3_data a b ca cb, caf) \notin Game5.prfkey_map{2})
-        => (msg1_data a b, ca) \notin NROc.RO.m{1})
-  /\ (forall a b ca cb, (forall caf, (msg3_data a b ca cb, caf) \notin Game5.prfkey_map{2})
-        => (msg2_data a b ca, cb) \notin NROc.RO.m{1})
-  /\ (forall a b ca cb caf, (msg3_data a b ca cb, caf) \in Game5.prfkey_map{2} =>
-         exists na nb, Game5.prfkey_map{2}.[(msg3_data a b ca cb, caf)] = Some (na, nb) /\
-                       NROc.RO.m{1}.[(msg1_data a b, ca)] = Some na /\
-                       NROc.RO.m{1}.[(msg2_data a b ca, cb)] = Some nb)
-  ) _ Game5_inv_test => //.
++ conseq (: ={res}
+          /\ ={b0, state_map, psk_map, dec_map, bad, nonce_map}(Game3c, Game3d)
+  ) _ Game3d_inv_send_msg2 => //.
+  by sim />.
+
++ conseq (: ={res}
+          /\ ={b0, state_map, psk_map, dec_map, bad, nonce_map}(Game3c, Game3d)
+  ) _ Game3d_inv_send_msg3 => //.
+  proc.
+  sp; if => //.
+  sp; match = => //.
+  + smt().
+  move => si m1.
+  sp; match = => //.
+  + by auto.
+  move => nb.
+  seq 1 1 : (#pre /\ ={cok}); 1: by auto.
+  sp; if => //.
+  rcondt {1} ^if.
+  + auto => />.
+    smt(mem_set).
+  rcondt {1} ^if.
+  + auto => />.
+    smt(mem_set).
+  by auto.
+
++ conseq (: ={res}
+          /\ ={b0, state_map, psk_map, dec_map, bad, nonce_map}(Game3c, Game3d)
+  ) _ Game3d_inv_send_fin => //.
+  proc.
+  sp; if => //.
+  sp; match = => //.
+  + smt().
+  move => sr m1 m2.
+  sp; match = => //.
+  + by auto.
+  move => nok.
+  rcondf {1} ^if.
+  + auto => />.
+    smt(mem_set).
+  rcondf {1} ^if.
+  + auto => />.
+    smt(mem_set).
+  by auto.
+
++ conseq (: ={res}
+          /\ ={b0, state_map, psk_map, dec_map, bad, nonce_map}(Game3c, Game3d)
+  ) _ Game3d_inv_reveal => //.
+  by sim />.
+
++ conseq (: ={res}
+          /\ ={b0, state_map, psk_map, dec_map, bad, nonce_map}(Game3c, Game3d)
+  ) _ Game3d_inv_test => //.
   by sim />.
 
 auto => />.
 smt(emptyE).
 qed.
 
+(* ------------------------------------------------------------------------------------------ *)
+(* Hop 9: Game 3d to Game 4 - Compress nonce map *)
+
+lemma Hop9 bit &m: Pr[AKE_Game(Game3d, A).run(bit) @ &m : res] = Pr[AKE_Game(Game4, A).run(bit) @ &m : res].
+byequiv => //.
+proc; inline.
+call (: ={b0, state_map, psk_map, dec_map, bad}(Game3d, Game4)
+      /\ (forall a b m1 m2 m3, (msg3_data a b m1 m2, m3) \in Game4.dec_map <=> (msg3_data a b m1 m2, m3) \in Game4.prfkey_map){2}
+      /\ (forall a b m1 m2 m3 n, Game4.prfkey_map{2}.[msg3_data a b m1 m2, m3] = Some n
+          => Game3d.nonce_map{1}.[msg1_data a b, m1] = Some n.`1
+            /\ Game3d.nonce_map{1}.[msg2_data a b m1, m2] = Some n.`2)
+      /\ (Game3d_inv Game3d.state_map Game3d.dec_map Game3d.nonce_map){1}
+); try by sim />.
+
++ conseq (: ={res}
+          /\ ={b0, state_map, psk_map, dec_map, bad}(Game3d, Game4)
+          /\ (forall a b m1 m2 m3, (msg3_data a b m1 m2, m3) \in Game4.dec_map <=> (msg3_data a b m1 m2, m3) \in Game4.prfkey_map){2}
+          /\ (forall a b m1 m2 m3 n, Game4.prfkey_map{2}.[msg3_data a b m1 m2, m3] = Some n
+              => Game3d.nonce_map{1}.[msg1_data a b, m1] = Some n.`1
+                /\ Game3d.nonce_map{1}.[msg2_data a b m1, m2] = Some n.`2)
+  ) Game3d_inv_send_msg1 => //.
+  proc.
+  sp; if => //.
+  auto => />.
+  smt(get_setE).
+  
++ conseq (: ={res}
+          /\ ={b0, state_map, psk_map, dec_map, bad}(Game3d, Game4)
+          /\ (forall a b m1 m2 m3, (msg3_data a b m1 m2, m3) \in Game4.dec_map <=> (msg3_data a b m1 m2, m3) \in Game4.prfkey_map){2}
+          /\ (forall a b m1 m2 m3 n, Game4.prfkey_map{2}.[msg3_data a b m1 m2, m3] = Some n
+              => Game3d.nonce_map{1}.[msg1_data a b, m1] = Some n.`1
+                /\ Game3d.nonce_map{1}.[msg2_data a b m1, m2] = Some n.`2)
+  ) Game3d_inv_send_msg2 => //.
+  proc.
+  sp; if => //.
+  match = => //.
+  + by auto.
+  move => na.
+  auto => />.
+  smt(get_setE).
+
++ conseq (: ={res}
+          /\ ={b0, state_map, psk_map, dec_map, bad}(Game3d, Game4)
+          /\ (forall a b m1 m2 m3, (msg3_data a b m1 m2, m3) \in Game4.dec_map <=> (msg3_data a b m1 m2, m3) \in Game4.prfkey_map){2}
+          /\ (forall a b m1 m2 m3 n, Game4.prfkey_map{2}.[msg3_data a b m1 m2, m3] = Some n
+              => Game3d.nonce_map{1}.[msg1_data a b, m1] = Some n.`1
+                /\ Game3d.nonce_map{1}.[msg2_data a b m1, m2] = Some n.`2)
+  ) Game3d_inv_send_msg3 => //.
+  proc.
+  sp; if => //.
+  sp; match = => //.
+  + smt().
+  move => si m1.
+  sp; match = => //.
+  + by auto.
+  move => nb.
+  seq 1 1 : (#pre /\ ={cok}); 1: by auto.
+  sp; if => //.
+  auto => />.
+  smt(get_setE).
+
++ conseq (: ={res}
+          /\ ={b0, state_map, psk_map, dec_map, bad}(Game3d, Game4)
+          /\ (forall a b m1 m2 m3, (msg3_data a b m1 m2, m3) \in Game4.dec_map <=> (msg3_data a b m1 m2, m3) \in Game4.prfkey_map){2}
+          /\ (forall a b m1 m2 m3 n, Game4.prfkey_map{2}.[msg3_data a b m1 m2, m3] = Some n
+              => Game3d.nonce_map{1}.[msg1_data a b, m1] = Some n.`1
+                /\ Game3d.nonce_map{1}.[msg2_data a b m1, m2] = Some n.`2)
+  ) Game3d_inv_send_fin => //.
++ proc.
+  sp; if => //.
+  sp; match = => //.
+  + smt().
+  move => sr m1 m2.
+  sp; match = => //.
+  + by auto.
+  move => nok.
+  auto => />.
+  smt(get_setE).
+
++ conseq (: ={res}
+          /\ ={b0, state_map, psk_map, dec_map, bad}(Game3d, Game4)
+          /\ (forall a b m1 m2 m3, (msg3_data a b m1 m2, m3) \in Game4.dec_map <=> (msg3_data a b m1 m2, m3) \in Game4.prfkey_map){2}
+          /\ (forall a b m1 m2 m3 n, Game4.prfkey_map{2}.[msg3_data a b m1 m2, m3] = Some n
+              => Game3d.nonce_map{1}.[msg1_data a b, m1] = Some n.`1
+                /\ Game3d.nonce_map{1}.[msg2_data a b m1, m2] = Some n.`2)
+  ) Game3d_inv_reveal => //.
+  by sim />.
+
++ conseq (: ={res}
+          /\ ={b0, state_map, psk_map, dec_map, bad}(Game3d, Game4)
+          /\ (forall a b m1 m2 m3, (msg3_data a b m1 m2, m3) \in Game4.dec_map <=> (msg3_data a b m1 m2, m3) \in Game4.prfkey_map){2}
+          /\ (forall a b m1 m2 m3 n, Game4.prfkey_map{2}.[msg3_data a b m1 m2, m3] = Some n
+              => Game3d.nonce_map{1}.[msg1_data a b, m1] = Some n.`1
+                /\ Game3d.nonce_map{1}.[msg2_data a b m1, m2] = Some n.`2)
+  ) Game3d_inv_test => //.
+  by sim />.
+
+auto => />.
+smt(emptyE).
+qed.
 
 (* ------------------------------------------------------------------------------------------ *)
-(* Step 5: Apply the PRF assumption. *)
+(* Hop 10: Game 4 to Game 5 - Apply the PRF assumption. *)
 
-lemma Step5 bit &m:
-    `|Pr[E_GAKE(Game5, A).run(bit) @ &m : res] - Pr[E_GAKE(Game6, A).run(bit) @ &m : res]|
+local clone import DProd.ProdSampling with
+  type t1 <- nonce,
+  type t2 <- nonce
+proof *.
+
+lemma Hop10 bit &m:
+    `|Pr[AKE_Game(Game4, A).run(bit) @ &m : res] - Pr[AKE_Game(Game5, A).run(bit) @ &m : res]|
   =
-    `|Pr[E_GPRF(PRF0, Red_PRF(A)).run(bit) @ &m : res] - Pr[E_GPRF(PRF1, Red_PRF(A)).run(bit) @ &m : res]|.
+    `|Pr[PRF_Game(PRF_Oracles_0, PRF_Reduction(A)).run(bit) @ &m : res] - Pr[PRF_Game(PRF_Oracles_1, PRF_Reduction(A)).run(bit) @ &m : res]|.
 proof.
 do! congr.
 + byequiv => //.
   proc; inline*.
   wp.
   call (:
-        ={b0, psk_map, state_map, dec_map, bad}(Game5, Red_PRF.WAKE_O)
-     /\ ={prfkey_map}(Game5, PRFb)
-     /\ (Game5_inv Game5.state_map Game5.dec_map Game5.prfkey_map){1}
-  )=> //.
+        ={b0, psk_map, state_map, dec_map, bad}(Game4, PRF_Reduction.R)
+     /\ Game4.prfkey_map{1} = PRF_Oracles_common.key_map{2}
+     /\ (forall a b m1 m2 m3, (msg3_data a b m1 m2, m3) \in Game4.dec_map <=> (msg3_data a b m1 m2, m3) \in Game4.prfkey_map){1}
+  ) => //.
 
   - by sim />.
 
-  - conseq (: ={res}
-     /\ ={psk_map, state_map, dec_map, bad}(Game5, Red_PRF.WAKE_O)
-     /\ ={prfkey_map}(Game5, PRFb)
-    ) Game5_inv_send_msg1 _ => //.
-   proc.
-   by sim />.
+  - proc.
+    sp; if => //.
+    auto => />.
+    smt(get_setE).
 
-  - conseq (: ={res}
-     /\ ={psk_map, state_map, dec_map, bad}(Game5, Red_PRF.WAKE_O)
-     /\ ={prfkey_map}(Game5, PRFb)
-    ) Game5_inv_send_msg2 _ => //.
-    by sim />.
+  - proc.
+    sp; if => //.
+    match = => //.
+    + by auto.
+    move => na.
+    auto => />.
+    smt(get_setE).
 
-  - conseq (: ={res}
-     /\ ={psk_map, state_map, dec_map, bad}(Game5, Red_PRF.WAKE_O)
-     /\ ={prfkey_map}(Game5, PRFb)
-    ) Game5_inv_send_msg3 _ => //.
-    proc; inline*.
-    sp; wp; if=> //.
+  - proc; inline.
+    sp; wp; if => //.
     sp; match = => //.
     + smt().
     move=> s m1.
     sp; match =.
     + smt().
-    + by auto=> />.
+    + by auto => />.
     move=> nb.
-    seq 1 1 : (#pre /\ ={caf}); 1: by auto.
+    seq 1 1 : (#pre /\ ={cok}); 1: by auto.
     sp; if=> //.
     rcondt{2} ^if.
     + auto=> />.
       smt().
     match Some {2} ^match.
     + by auto => />; smt(mem_set get_setE).
+    outline {2} ^k0<$ ~ ProdSampling.S.sample.
+    rewrite equiv [{2} ^ <@ ProdSampling.sample_sample2].
+    inline.
     auto => />.
     smt(get_setE).
 
-  - conseq (: ={res}
-     /\ ={psk_map, state_map, dec_map, bad}(Game5, Red_PRF.WAKE_O)
-     /\ ={prfkey_map}(Game5, PRFb)
-    ) Game5_inv_send_fin _ => //.
-     proc; inline*.
-     sp; wp ^if ^if; if=> //.
-     sp; match = => //.
-     + smt().
-     move=> s m1 m2.
-     sp; match =.
-     + smt().
-     + by auto=> />.
-     move=> nok.
-     match Some {2} ^match.
-     + auto=> />.
-       smt().
-     auto => />.
-     smt(get_setE).
+  - proc; inline*.
+    sp; wp ^if ^if; if=> //.
+    sp; match = => //.
+    + smt().
+    move=> s m1 m2.
+    sp; match =.
+    + smt().
+    + by auto=> />.
+    move=> nok.
+    match Some {2} ^match.
+    + auto=> />.
+      smt().
+    auto => />.
+    smt(get_setE).
 
-  - conseq (: ={res}
-     /\ ={psk_map, state_map, dec_map, bad}(Game5, Red_PRF.WAKE_O)
-     /\ ={prfkey_map}(Game5, PRFb)
-    ) Game5_inv_reveal _ => //.
     by sim />.
 
-  - conseq (: ={res}
-     /\ ={psk_map, state_map, dec_map, bad}(Game5, Red_PRF.WAKE_O)
-     /\ ={prfkey_map}(Game5, PRFb)
-    ) Game5_inv_test _ => //.
     by sim />.
 
   auto => />.
@@ -1540,11 +1662,11 @@ byequiv => //.
 proc; inline *.
 wp.
 call (:
-      ={b0, psk_map, state_map, dec_map, bad}(Game6, Red_PRF.WAKE_O)
-   /\ ={prfkey_map}(Game6, PRFb)
-   /\ (forall a b m1 m2 m3, ((a, b), msg3_data a b m1 m2, m3) \in Game6.dec_map{1} <=> ((msg3_data a b m1 m2, m3), (a, b)) \in PRF1.cache{2})
-   /\ (forall a b m1 m2 m3 k, PRF1.cache.[((msg3_data a b m1 m2, m3), (a, b))]{2} = Some k => Game6.sk_map.[((a, m1), m2, m3)]{1} = Some k)
-   /\ (forall a b m1 m2 m3, ((a, b), msg3_data a b m1 m2, m3) \in Game6.dec_map <=> (msg3_data a b m1 m2, m3) \in Game6.prfkey_map){1}
+      ={b0, psk_map, state_map, dec_map, bad}(Game5, PRF_Reduction.R)
+     /\ Game5.prfkey_map{1} = PRF_Oracles_common.key_map{2}
+   /\ (forall a b m1 m2 m3, (msg3_data a b m1 m2, m3) \in Game5.dec_map{1} <=> ((msg3_data a b m1 m2, m3), (a, b)) \in PRF_Oracles_1.cache{2})
+   /\ (forall a b m1 m2 m3 k, PRF_Oracles_1.cache.[(msg3_data a b m1 m2, m3), (a, b)]{2} = Some k => Game5.key_map.[(a, m1), m2, m3]{1} = Some k)
+   /\ (forall a b m1 m2 m3, (msg3_data a b m1 m2, m3) \in Game5.dec_map <=> (msg3_data a b m1 m2, m3) \in Game5.prfkey_map){1}
 )=> //.
 
 - by sim />.
@@ -1562,44 +1684,47 @@ call (:
   smt(get_setE).
 
 - proc; inline*.
-  sp; wp; if=> //.
+  sp; wp; if => //.
   sp; match = => //.
   + smt().
-  move=> s m1.
+  move => s m1.
   sp; match =.
   + smt().
   + by auto=> />.
-  move=> nb.
-  seq 1 1 : (#pre /\ ={caf}); 1: by auto.
-  sp; if=> //.
-  rcondt{2} ^if.
-  + auto=> />.
-    smt().
-  match Some {2} ^match.
-  + auto=> />.
-    smt(get_setE).
+  move => nb.
+  seq 1 1 : (#pre /\ ={cok}); 1: by auto.
+  sp; if => //.
   rcondt{2} ^if.
   + auto => />.
     smt().
-  auto=> />.
+  match Some {2} ^match.
+  + auto => />.
+    smt(get_setE).
+  outline {2} ^k0<$ ~ ProdSampling.S.sample.
+  rewrite equiv [{2} ^ <@ ProdSampling.sample_sample2].
+  inline.
+  rcondt{2} ^if.
+  + auto => />.
+    smt().
+  auto => />.
   smt(get_setE).
 
 - proc; inline*.
-  sp; wp ^if ^if; if=> //.
+  sp; wp ^if ^if; if => //.
   sp; match = => //.
   + smt().
   move=> s m1 m2.
   sp; match =.
   + smt().
-  + by auto=> />.
-  move=> nok.
+  + by auto => />.
+  move => nok.
   match Some {2} ^match.
-  + auto=> />.
+  + auto => />.
     smt().
   rcondf{2} ^if.
   + auto => />.
     smt().
-  auto=> />.
+  auto => />.
   smt().
 
 - by sim />.
@@ -1611,9 +1736,9 @@ smt(emptyE).
 qed.
 
 (* ------------------------------------------------------------------------------------------ *)
-(* Step 6: Remove skeys from the state using sk_map to retrieve. *)
+(* Hop 11: Game 5 to Game 5a - Remove skeys from the state using key_map to retrieve. *)
 
-local op clear_sk (s : instance_state) =
+local op clean3 (s : session_state) =
 match s with
 | IPending _ _ => s
 | RPending _ _ _ => s
@@ -1622,43 +1747,34 @@ match s with
 | Aborted   => s
 end.
 
-local lemma eq_partners_sk tr r sml smr:
-  (forall h, omap (fun (v: role * instance_state) => let (r, s) = v in (r, clear_sk s)) sml.[h] = smr.[h]) =>
-get_partners tr r sml = get_partners tr r smr.
+local lemma clean3_fresh h sml smr:
+  (forall h, omap (fun (v: _ * _) => let (r, s) = v in (r, clean3 s)) sml.[h] = smr.[h]) =>
+  fresh h sml <=> fresh h smr.
 proof.
-move=> eqsm.
-rewrite /get_partners fsetP => h'.
-rewrite !mem_fdom !mem_filter !domE /#.
+move=> eq_sm.
+rewrite /fresh.
+have eq_ps : partners h sml = partners h smr.
++ rewrite /get_partners fsetP => h'.
+  by rewrite !mem_fdom !mem_filter !domE /#.
+rewrite /observed_partners eq_ps.
+do! congr.
+rewrite fun_ext => h'.
+rewrite -(eq_sm h') //=.
+case: (sml.[h'])=> //.
+by move => [r' []] // [].
 qed.
 
-local lemma eq_obs_partners_sk h sml smr:
-  (forall h, omap (fun (v: role * instance_state) => let (r, s) = v in (r, clear_sk s)) sml.[h] = smr.[h]) =>
-get_observed_partners h sml = get_observed_partners h smr.
-proof.
-move=> eqsm.
-rewrite /get_observed_partners.
-congr.
-+ rewrite fun_ext => bj.
-  rewrite -(eqsm bj) //=.
-  case: (sml.[bj])=> //.
-  by move=> [r' []] // [].
-rewrite -(eq_partners_sk _ _ sml smr eqsm).
-rewrite -(eqsm h) /s /r //=.
-case: (sml.[h])=> //.
-by move=> [r' []] // [].
-qed.
-
-lemma Step6 bit &m:
-    Pr[E_GAKE(Game6, A).run(bit) @ &m : res] = Pr[E_GAKE(Game7, A).run(bit) @ &m : res].
+lemma Hop11 bit &m:
+    Pr[AKE_Game(Game5, A).run(bit) @ &m : res] = Pr[AKE_Game(Game5a, A).run(bit) @ &m : res].
 proof.
 byequiv => //.
 proc; inline*.
 call (:
-    ={b0, psk_map, dec_map, bad, prfkey_map, sk_map}(Game6, Game7)
-/\ (forall h, omap (fun v => let (r, s) = v in (r, clear_sk s)) Game6.state_map.[h]{1} = Game7.state_map.[h]{2})
-/\ (forall h r tr k, Game6.state_map.[h] = Some (r, Accepted tr k) => Game6.sk_map.[tr] = Some k){1}
-/\ (forall a b m1 m2 m3, ((a, b), msg3_data a b m1 m2, m3) \in Game6.dec_map => ((a, m1), m2, m3) \in Game6.sk_map){1}
-/\ (forall m, (forall pk ad , (pk, ad, m) \notin Game6.dec_map) => (forall a m1 m2 m3, ((a, m1), m2, m3) \in Game6.sk_map => m3 <> m)){1}
+    ={b0, psk_map, dec_map, bad, prfkey_map, key_map}(Game5, Game5a)
+/\ (forall h, omap (fun v => let (r, s) = v in (r, clean3 s)) Game5.state_map.[h]{1} = Game5a.state_map.[h]{2})
+/\ (forall h r tr k, Game5.state_map.[h] = Some (r, Accepted tr k) => Game5.key_map.[tr] = Some k){1}
+/\ (forall a b m1 m2 m3, (msg3_data a b m1 m2, m3) \in Game5.dec_map => ((a, m1), m2, m3) \in Game5.key_map){1}
+/\ (forall m, (forall ad , (ad, m) \notin Game5.dec_map) => (forall a m1 m2 m3, ((a, m1), m2, m3) \in Game5.key_map => m3 <> m)){1}
 ).
 
 - by sim />.
@@ -1679,110 +1795,111 @@ call (:
   smt(mem_set get_setE).
 
 - proc; inline*.
-  sp; wp; if=> //.
+  sp; wp; if => //.
   + smt().
-  sp; match; 1..5: smt(); 2..5: by auto.
-  move=> sl m1l sr m1r.
+  sp; match; 1..5: smt(); ~1: by auto.
+  move => sl m1l sr m1r.
   sp; match =.
   + smt().
   + auto=> />.
     smt(get_setE).
   move=> nb.
-  seq 1 1 : (#pre /\ ={caf}); 1: by auto.
-  sp; if=> //.
-  auto=> />.
+  seq 1 1 : (#pre /\ ={cok}); 1: by auto.
+  sp; if => //.
+  auto => />.
   smt(mem_set get_setE).
 
 - proc; inline*.
-  sp; wp ^if ^if; if=> //.
+  sp; wp ^if ^if; if => //.
   + smt().
-  sp; match; 1..5: smt(); 1,3..5: by auto.
-  move=> sl m1l m2l sr m1r m2r.
+  sp; match; 1..5: smt(); ~2: by auto.
+  move => sl m1l m2l sr m1r m2r.
   sp; match =.
   + smt().
   + auto=> />.
     smt(get_setE).
-  move=> nok.
-  auto=> />.
+  move => nok.
+  auto => />.
   smt(get_setE).
 
 - proc; inline.
-  sp; wp ^if ^if; if=> //.
+  sp; wp ^if ^if; if => //.
   + smt().
-  sp; match; 1..5: smt(); 1,2,4,5: by auto.
+  sp; match; 1..5: smt(); ~3: by auto.
   move=> tr k tr' k'.
-  sp ^if & -1 ^if & -1; if=> //.
-  + move => &1 &2 [] /> *.
-    by rewrite (eq_obs_partners_sk (a, i){2} Game6.state_map{1} Game7.state_map{2}) => //.
+  sp ^if & -1 ^if & -1; if => //.
+  + move => &1 &2 [] |> *.
+    by rewrite (clean3_fresh h{2} Game5.state_map{1} Game5a.state_map{2}).
   auto=> /> &1 &2 + + eqsm invl a_in _.
-  rewrite -(eqsm (a, i){2}).
+  rewrite -(eqsm h{2}).
   move => *.
-  split. smt().
+  split; 1: smt().
   split.
-  move => h.
-  case (h = (a, i){2}) => [|hneq].
-  smt(get_set_sameE).
-  do rewrite get_set_neqE => //. rewrite eqsm => //.
+  move => h'.
+  case (h' = h{2}) => [|hneq].
+  + smt(get_set_sameE).
+  rewrite !get_set_neqE // eqsm //.
   smt(get_setE).
 
 - proc; inline.
-  sp; wp ^if ^if; if=> //.
+  sp; wp ^if ^if; if => //.
   + smt().
-  sp; match; 1..5: smt(); 1,2,4,5: by auto.
+  sp; match; 1..5: smt(); ~3: by auto.
   move=> tr k tr' k'.
-  sp ^if & -1 ^if & -1; if=> //.
-  + move => &1 &2 [] /> *.
-    by rewrite (eq_obs_partners_sk (a, i){2} Game6.state_map{1} Game7.state_map{2}) => //.
+  sp ^if & -1 ^if & -1; if => //.
+  + move => &1 &2 [] |> *.
+    by rewrite (clean3_fresh h{2} Game5.state_map{1} Game5a.state_map{2}).
   if => //.
   + auto=> /> &1 &2 + + eqsm invl a_in _.
-    rewrite -(eqsm (a, i){2}).
+    rewrite -(eqsm h{2}).
     move => *.
-    split. smt().
+    split; 1: smt().
     split.
-    move => h.
-    case (h = (a, i){2}) => [|hneq].
+    move => h'.
+    case (h' = h{2}) => [|hneq].
     + smt(get_set_sameE).
-    do rewrite get_set_neqE => //. rewrite eqsm => //.
+    rewrite !get_set_neqE // eqsm //.
     smt(get_setE).
-  auto=> /> &1 &2 + + eqsm invl a_in _ _ _ ideal sk _.
-  rewrite -(eqsm (a, i){2}).
+  auto => /> &1 &2 + + eqsm invl a_in _ _ _ ? ideal sk _.
+  rewrite -(eqsm h{2}).
   move => stm1 stm2.
-  split. move => h.
-  case (h = (a, i){2}) => [|hneq].
+  split; 2: smt(get_setE).
+  move => h'.
+  case (h' = h{2}) => [|hneq].
   + smt(get_set_sameE).
-  do rewrite get_set_neqE => //. rewrite eqsm => //.
-  smt(get_setE).
+  by rewrite !get_set_neqE // eqsm.
 
-auto=> />.
+auto => />.
 by smt(emptyE).
 qed.
 
 (* ------------------------------------------------------------------------------------------ *)
-(* Step 7: Delaying sampling of the keys to reveal/test *)
-lemma Step7 &m b:
-    Pr[E_GAKE(Game7, A).run(b) @ &m : res] = Pr[E_GAKE(Game8, A).run(b) @ &m : res].
+(* Hop 12: Game 5a to Game 5b - Delaying sampling of the keys to reveal/test *)
+
+lemma Hop12 &m b:
+    Pr[AKE_Game(Game5a, A).run(b) @ &m : res] = Pr[AKE_Game(Game5b, A).run(b) @ &m : res].
 proof.
 byequiv => //.
 proc*.
 
 (* Proof for the real side *)
-transitivity* {1} { r <@ KROc.MainD(Red_ROM_sk(A), KROc.RO).distinguish(b); }.
+transitivity* {1} { r <@ KROc.MainD(Key_Delay_Reduction(A), KROc.RO).distinguish(b); }.
 + inline*; wp.
-  call(: ={b0, state_map, psk_map, dec_map, bad, prfkey_map}(Game7, Red_ROM_sk.WAKE_O)
-         /\ Game7.sk_map{1} = KROc.RO.m{2}
-  /\ (forall h r tr k, Game7.state_map.[h] = Some (r, Accepted tr k) => tr \in Game7.sk_map){1}
-  /\ (forall a b m1 m2 m3, ((a, b), msg3_data a b m1 m2, m3) \in Game7.dec_map => ((a, m1), m2, m3) \in Game7.sk_map){1}
-  /\ (forall m1 m2 m3, (forall pk ad, (pk, ad, m3) \notin Game7.dec_map) => (m1, m2, m3) \notin Game7.sk_map){1}
+  call(: ={b0, state_map, psk_map, dec_map, bad, prfkey_map}(Game5a, Key_Delay_Reduction.R)
+         /\ Game5a.key_map{1} = KROc.RO.m{2}
+         /\ (forall h r tr k, Game5a.state_map.[h] = Some (r, Accepted tr k) => tr \in Game5a.key_map){1}
+         /\ (forall a b m1 m2 m3, (msg3_data a b m1 m2, m3) \in Game5a.dec_map => ((a, m1), m2, m3) \in Game5a.key_map){1}
+         /\ (forall m1 m2 m3, (forall ad, (ad, m3) \notin Game5a.dec_map) => (m1, m2, m3) \notin Game5a.key_map){1}
   ).
 
   - by sim />.
 
-  - proc; inline*.
+  - proc; inline.
     sp; wp; if => //.
     auto => />.
     smt(mem_set get_setE).
 
-  - proc; inline*.
+  - proc; inline.
     sp; wp; if => //.
     match = => //.
     + auto => />.
@@ -1790,87 +1907,81 @@ transitivity* {1} { r <@ KROc.MainD(Red_ROM_sk(A), KROc.RO).distinguish(b); }.
     auto => />.
     smt(mem_set get_setE).
 
-  - proc; inline*.
-    sp; wp; if=> //.
+  - proc; inline.
+    sp; wp; if => //.
     sp; match = => //.
     + smt().
     move=> s m1.
     sp; match =.
     + smt().
-    + auto=> />.
+    + auto => />.
       smt(get_setE).
-    move=> nb.
-    seq 1 1 : (#pre /\ ={caf}); 1: by auto.
-    sp; if=> //.
-    auto=> />.
+    move => nb.
+    seq 1 1 : (#pre /\ ={cok}); 1: by auto.
+    sp; if => //.
+    rcondt {2} ^if.
+    + by auto => /#.
+    wp.
+    rnd.
+    wp; rnd{2}.
+    auto => />.
     smt(mem_set get_setE).
 
-  - proc; inline*.
-    sp; wp ^if ^if; if=> //.
+  - proc; inline.
+    sp; wp ^if ^if; if => //.
     sp; match = => //.
     + smt().
-    move=> s m1 m2.
+    move => s m1 m2.
     sp; match = => //.
-    + auto=> />.
+    + auto => />.
       smt(get_setE).
-    move=> nok.
-    auto=> />.
+    move => nok.
+    auto => />.
     smt(get_setE).
 
-  - proc; inline*.
+  - proc; inline.
     sp; wp ^if ^if; if => //.
     sp 1 1; match = => //.
     + smt().
-    move=> tr k'.
-    sp ^if & -1 ^if & -1; if => //.
-    rcondf {2} 3; 1: by auto => /#.
-    kill {2} ^r<$; 1: by islossless.
-    auto=> /> &1 &2.
+    move => tr k'.
+    if => //.
+    auto => />.
     smt(get_setE).
 
-  - proc; inline*.
+  - proc; inline.
     sp; wp ^if ^if; if => //.
     sp 1 1; match = => //.
     + smt().
-    move=> tr k'.
-    sp ^if & -1 ^if & -1; if=> //.
-    rcondf {2} ^if; 1: by auto => /#.
-    if{1}.
-    + rcondf {2} ^if; 1: by auto => /#.
-      auto=> /> &1 &2.
+    move => tr k'.
+    if => //.
+    rcondf{2} ^if.
+    + auto => />.
       smt(get_setE).
-    rcondt {2} ^if; 1: by auto => /#.
-    auto=> /> &1 &2.
-    smt(get_setE).
-
-  auto=> />.
+    kill{2} ^r0<$; 1: islossless.
+    by sp; if; auto; smt(get_setE).
+    
+  auto => />.
   smt(emptyE).
 
-rewrite equiv [{1} 1 (KROc.FullEager.RO_LRO (Red_ROM_sk(A)) _)]; 1: by move=> _; exact dskey_ll.
+rewrite equiv [{1} 1 (KROc.FullEager.RO_LRO (Key_Delay_Reduction(A)) _)]; 1: by move=> _; exact dskey_ll.
++ auto => />.
 inline; wp.
-sim (: ={state_map, psk_map, dec_map, bad, prfkey_map}(Red_ROM_sk.WAKE_O, Game8)
-     /\ Red_ROM_sk.WAKE_O.b0{1} = Game8.b0{2}
-     /\ KROc.RO.m{1} = Game8.sk_map{2}
+sim (: ={state_map, psk_map, dec_map, bad, prfkey_map}(Key_Delay_Reduction.R, Game5b)
+     /\ Key_Delay_Reduction.R.b0{1} = Game5b.b0{2}
+     /\ KROc.RO.m{1} = Game5b.key_map{2}
 ).
 
 - proc; inline.
   sp; if => //.
-  sp; match = => //.
+  sp.
+  match = => //.
   + smt().
   move => tr k'.
-  sp ^if & -1 ^if & -1; if => //.
-  sp; seq 1 1 : (#pre /\ r{1} = k''{2}); 1: by auto => />.
-  case (Game8.b0{2}).
-  + rcondt {1} ^if{2}; 1: by auto => /#.
-    rcondf {2} ^if{2}; 1: by auto => /#.
-    sim.
-    auto.
-    smt(get_setE).
-  rcondf {1} ^if{2}; 1: by auto => /#.
-  rcondt {2} ^if{2}; 1: by auto => /#.
-  sim.
-  auto.
-  smt(get_setE).
+  if => //.
+  sp; seq 1 1 : (#pre /\ r0{1} = k'{!2}); 1: by auto.
+  if => //.
+  + by sp; if; auto; smt(get_setE).
+  by sp; if; auto; smt(get_setE).
 
 - proc; inline.
   sp; if => //.
@@ -1878,9 +1989,7 @@ sim (: ={state_map, psk_map, dec_map, bad, prfkey_map}(Red_ROM_sk.WAKE_O, Game8)
   + smt().
   move => tr k'.
   sp ^if & -1 ^if & -1; if => //.
-  sp; seq 1 1 : (#pre /\ r{1} = k''{2}); 1: by auto => />.
-  sim.
-  auto.
+  auto => />.
   smt(get_setE).
 
 - proc; inline.
@@ -1891,122 +2000,102 @@ sim (: ={state_map, psk_map, dec_map, bad, prfkey_map}(Red_ROM_sk.WAKE_O, Game8)
   sp; match = => //.
   + by auto.
   move => nb.
-  seq 1 1 : (#pre /\ ={caf}); 1: by auto.
+  seq 1 1 : (#pre /\ ={cok}); 1: by auto.
   sp; if => //.
-  by auto.
+  wp; rnd{1}.
+  by auto => />.
 
 by auto.
 qed.
 
 (* ------------------------------------------------------------------------------------------ *)
-(* Step 8: Replace sampling derived from the sk_map to a fresh sample in test *)
-lemma Step8 &m:
-    Pr[E_GAKE(Game8, A).run(false) @ &m : res] = Pr[E_GAKE(Game8, A).run(true) @ &m : res].
+(* Hop 13: Game 5b to Game 3c - Remove checks for new key samplings *)
+
+
+lemma Hop13 &m b:
+    Pr[AKE_Game(Game5b, A).run(b) @ &m : res] = Pr[AKE_Game(Game5c, A).run(b) @ &m : res].
 proof.
 byequiv => //.
 proc; inline.
-call (: ={state_map, psk_map, dec_map, bad, prfkey_map}(Game8, Game8)
-     /\ !Game8.b0{1} /\ Game8.b0{2}
-     /\ (forall h, h \in Game8.sk_map{1} <=> h \in Game8.sk_map{2})
-     /\ (Game8_inv Game8.state_map Game8.dec_map Game8.sk_map){1}
+call (: ={state_map, psk_map, b0, dec_map, bad, prfkey_map, key_map}(Game5b, Game5c)
+     /\ (Game5c_inv Game5c.state_map Game5c.dec_map Game5c.key_map){2}
 ).
 
 - by sim />.
 
 - conseq (: ={res}
-     /\ ={state_map, psk_map, dec_map, bad, prfkey_map}(Game8, Game8)
-     /\ !Game8.b0{1} /\ Game8.b0{2}
-     /\ (forall h, h \in Game8.sk_map{1} <=> h \in Game8.sk_map{2})
-  ) Game8_inv_send_msg1 _ => //.
+     /\ ={state_map, psk_map, b0, dec_map, bad, prfkey_map, key_map}(Game5b, Game5c)
+  ) _ Game5c_inv_send_msg1 => //.
+  by sim />.
+- conseq (: ={res}
+     /\ ={state_map, psk_map, b0, dec_map, bad, prfkey_map, key_map}(Game5b, Game5c)
+  ) _ Game5c_inv_send_msg2 => //.
+  by sim />.
+- conseq (: ={res}
+     /\ ={state_map, psk_map, b0, dec_map, bad, prfkey_map, key_map}(Game5b, Game5c)
+  ) _ Game5c_inv_send_msg3 => //.
+  by sim />.
+- conseq (: ={res}
+     /\ ={state_map, psk_map, b0, dec_map, bad, prfkey_map, key_map}(Game5b, Game5c)
+  ) _ Game5c_inv_send_fin => //.
   by sim />.
 
 - conseq (: ={res}
-     /\ ={state_map, psk_map, dec_map, bad, prfkey_map}(Game8, Game8)
-     /\ !Game8.b0{1} /\ Game8.b0{2}
-     /\ (forall h, h \in Game8.sk_map{1} <=> h \in Game8.sk_map{2})
-  ) Game8_inv_send_msg2 _ => //.
-  by sim />.
-
-- conseq (: ={res}
-     /\ ={state_map, psk_map, dec_map, bad, prfkey_map}(Game8, Game8)
-     /\ !Game8.b0{1} /\ Game8.b0{2}
-     /\ (forall h, h \in Game8.sk_map{1} <=> h \in Game8.sk_map{2})
-  ) Game8_inv_send_msg3 _ => //.
-  by sim />.
-
-- conseq (: ={res}
-     /\ ={state_map, psk_map, dec_map, bad, prfkey_map}(Game8, Game8)
-     /\ !Game8.b0{1} /\ Game8.b0{2}
-     /\ (forall h, h \in Game8.sk_map{1} <=> h \in Game8.sk_map{2})
-  ) Game8_inv_send_fin _ => //.
-  by sim />.
-
-- conseq (: ={res}
-     /\ ={state_map, psk_map, dec_map, bad, prfkey_map}(Game8, Game8)
-     /\ !Game8.b0{1} /\ Game8.b0{2}
-     /\ (forall h, h \in Game8.sk_map{1} <=> h \in Game8.sk_map{2})
-  ) Game8_inv_reveal _ => //.
-  proc; inline*.
+     /\ ={state_map, psk_map, b0, dec_map, bad, prfkey_map, key_map}(Game5b, Game5c)
+  ) _ Game5c_inv_reveal => //.
+  proc; inline.
   sp; wp ^if ^if; if => //.
   sp 1 1; match = => //.
   + smt().
   move=> tr k'.
   sp ^if & -1 ^if & -1; if => //.
-  seq 1 1 : (={k''} /\ #pre); 1: by auto => />.
+  seq 1 1 : (={k'} /\ #pre); 1: by auto => />.
   if{1}.
-  + rcondt {2} ^if; 1: by auto => /#.
-    auto => />.
-    smt(get_setE).
+  + by auto => /#.
   exfalso.
   move => &1 &2 [#] />.
-  move => smai2 smai1 _ _. 
-  move => _ uniq_pi ss_log_ip ss_log_rp ss_log_acc ss_log_obs sk_obs ai_in obs_ps.
-  case (tr \in Game8.sk_map{1}) => // ^ tr_in_skm.
+  move => smai2 smai1. 
+  move => uniq_pi ss_log_rp ss_log_ip ss_log_acc ss_log_obs sk_obs ai_in _ obs_ps.
+  case (tr \in Game5c.key_map{2}) => // ^ tr_in_skm.
   move => /(sk_obs tr) [a' i' r sk smai'].
-  have smai : Game8.state_map{2}.[a{2}, i{2}] = Some (role{1}, Accepted tr k') by smt().
-  case (r = role{1}).
-  + have := uniq_pi tr.`1.`2 r (a, i){2} (Accepted tr k'){m} (a', i') (Observed tr sk).
+  have smai : Game5c.state_map.[h]{2} = Some (r{!2}, Accepted tr k') by smt().
+  case (r = r{!2}).
+  + have := uniq_pi tr.`1.`2 r h{2} (Accepted tr k') (a', i') (Observed tr sk).
     smt().
   move => neq_role.
-  have bj_partner : (a', i') \in get_partners (Some tr) role{1} Game8.state_map{2}.
+  have bj_partner : (a', i') \in partners h{2} Game5c.state_map{2}.
   + rewrite /get_partners mem_fdom mem_filter /#.
-  have // : (a', i') \in get_observed_partners (a, i){2} Game8.state_map{2}.
+  have // : (a', i') \in observed_partners h{2} Game5c.state_map{2}.
   + rewrite /get_observed_partners in_filter /#.
   rewrite fcard_eq0 in obs_ps.
   by rewrite obs_ps in_fset0.
 
 - conseq (: ={res}
-     /\ ={state_map, psk_map, dec_map, bad, prfkey_map}(Game8, Game8)
-     /\ !Game8.b0{1} /\ Game8.b0{2}
-     /\ (forall h, h \in Game8.sk_map{1} <=> h \in Game8.sk_map{2})
-  ) Game8_inv_test _ => //.
+     /\ ={state_map, psk_map, b0, dec_map, bad, prfkey_map, key_map}(Game5b, Game5c)
+  ) _ Game5c_inv_test => //.
   proc; inline*.
   sp; wp ^if ^if; if => //.
   sp 1 1; match = => //.
   + smt().
   move=> tr k'.
-  sp ^if & -1 ^if & -1; if => //.
-  rcondt {1} ^if{2}; 1: by auto => /#.
-  rcondf {2} ^if{2}; 1: by auto => /#.
-  case (tr \notin Game8.sk_map{1}).
-  + rcondt {1} ^if; 1: by auto => />.
-    rcondt {2} ^if; 1: by auto => /#.
-    auto => />.
-    smt(get_setE).
+  if => //.
+  seq 1 1 : (={k'} /\ #pre); 1: by auto => />.
+  if{1}.
+  + by sp; if; auto => /#.
   exfalso.
   move => &1 &2 [#] />.
-  move => smai2 smai1 _ _. 
-  move => _ uniq_pi ss_log_ip ss_log_rp ss_log_acc ss_log_obs sk_obs ai_in obs_ps.
-  case (tr \in Game8.sk_map{1}) => // ^ tr_in_skm.
+  move => smai2 smai1. 
+  move => uniq_pi ss_log_rp ss_log_ip ss_log_acc ss_log_obs sk_obs ai_in _ obs_ps.
+  case (tr \in Game5c.key_map{2}) => // ^ tr_in_skm.
   move => /(sk_obs tr) [a' i' r sk smai'].
-  have smai: Game8.state_map{2}.[a{2}, i{2}] = Some (role{1}, Accepted tr k') by smt().
-  case (r = role{1}).
-  + have := uniq_pi tr.`1.`2 r (a, i){2} (Accepted tr k'){m} (a', i') (Observed tr sk).
+  have smai : Game5c.state_map.[h]{2} = Some (r{!2}, Accepted tr k') by smt().
+  case (r = r{!2}).
+  + have := uniq_pi tr.`1.`2 r h{2} (Accepted tr k') (a', i') (Observed tr sk).
     smt().
   move => neq_role.
-  have bj_partner : (a', i') \in get_partners (Some tr) role{1} Game8.state_map{2}.
+  have bj_partner : (a', i') \in partners h{2} Game5c.state_map{2}.
   + rewrite /get_partners mem_fdom mem_filter /#.
-  have // : (a', i') \in get_observed_partners (a, i){2} Game8.state_map{2}.
+  have // : (a', i') \in observed_partners h{2} Game5c.state_map{2}.
   + rewrite /get_observed_partners in_filter /#.
   rewrite fcard_eq0 in obs_ps.
   by rewrite obs_ps in_fset0.
@@ -2015,36 +2104,69 @@ auto => />.
 smt(emptyE mem_empty).
 qed.
 
+(* ------------------------------------------------------------------------------------------ *)
+(* Hop 14: Game 5c to Game 5c - flip the bit *)
 
-lemma final &m: `| Pr[E_GAKE(GAKEb(NSL), A).run(false) @ &m : res] - Pr[E_GAKE(GAKEb(NSL), A).run(true) @ &m : res]|
-  <= `|Pr[E_GAEAD(GAEAD0, Red_AEAD(A)).run(false) @ &m : res] - Pr[E_GAEAD(GAEAD1, Red_AEAD(A)).run(false) @ &m : res]|
-      + `|Pr[E_GAEAD(GAEAD0, Red_AEAD(A)).run(true) @ &m : res] - Pr[E_GAEAD(GAEAD1, Red_AEAD(A)).run(true) @ &m : res]|
-      + `|Pr[E_GPRF(PRF0, Red_PRF(A)).run(false) @ &m : res] - Pr[E_GPRF(PRF1, Red_PRF(A)).run(false) @ &m : res]|
-      + `|Pr[E_GPRF(PRF0, Red_PRF(A)).run(true) @ &m : res] - Pr[E_GPRF(PRF1, Red_PRF(A)).run(true) @ &m : res]|
+lemma Hop14 &m:
+    Pr[AKE_Game(Game5c, A).run(false) @ &m : res] = Pr[AKE_Game(Game5c, A).run(true) @ &m : res].
+proof.
+byequiv => //.
+proc; inline.
+call (: ={state_map, psk_map, dec_map, bad, prfkey_map}(Game5c, Game5c)
+     /\ !Game5c.b0{1} /\ Game5c.b0{2}
+     /\ (forall h, h \in Game5c.key_map{1} <=> h \in Game5c.key_map{2})
+); try by sim />.
+
++ proc; inline*.
+  sp; if => //.
+  sp; match = => //.
+  + smt().
+  move=> tr k'.
+  if => //.
+  auto => />.
+  smt(get_setE).
+
++ proc; inline*.
+  sp; if => //.
+  sp; match = => //.
+  + smt().
+  move=> tr k'.
+  if => //.
+  rcondt{1} ^if; 1: by auto => />.
+  rcondf{2} ^if; 1: by auto => />.
+  auto => />.
+  smt(get_setE).
+
+by auto => />.
+qed.
+
+lemma final &m: `| Pr[AKE_Game(AKE_Oracles(NSL), A).run(false) @ &m : res] - Pr[AKE_Game(AKE_Oracles(NSL), A).run(true) @ &m : res]|
+  <= `|Pr[AEAD_Game(AEAD_Oracles_0, AEAD_Reduction(A)).run(false) @ &m : res] - Pr[AEAD_Game(AEAD_Oracles_1, AEAD_Reduction(A)).run(false) @ &m : res]|
+      + `|Pr[AEAD_Game(AEAD_Oracles_0, AEAD_Reduction(A)).run(true) @ &m : res] - Pr[AEAD_Game(AEAD_Oracles_1, AEAD_Reduction(A)).run(true) @ &m : res]|
+      + `|Pr[PRF_Game(PRF_Oracles_0, PRF_Reduction(A)).run(false) @ &m : res] - Pr[PRF_Game(PRF_Oracles_1, PRF_Reduction(A)).run(false) @ &m : res]|
+      + `|Pr[PRF_Game(PRF_Oracles_0, PRF_Reduction(A)).run(true) @ &m : res] - Pr[PRF_Game(PRF_Oracles_1, PRF_Reduction(A)).run(true) @ &m : res]|
       + 2%r * ((q_m1 + q_m2 + q_m3) ^ 2)%r * mu1 dctxt (mode dctxt).
 proof.
-rewrite !Step0.
-do rewrite - Step1 -Step5 Step6 -Step4 -Step3.
+do rewrite Hop1 Hop2.
+do rewrite -Hop3 -Hop10.
+do rewrite -Hop9 -Hop8 -Hop7 -Hop6 -Hop5.
+do rewrite Hop11 Hop12 Hop13.
 apply (StdOrder.RealOrder.ler_trans
-        (`|Pr[E_GAKE(Game1, A).run(false) @ &m : res] -
-  Pr[E_GAKE(Game2, A).run(false) @ &m : res]| +
-`|Pr[E_GAKE(Game1, A).run(true) @ &m : res] -
-  Pr[E_GAKE(Game2, A).run(true) @ &m : res]| +
-`|Pr[E_GAKE(Game2, A).run(false) @ &m : res] -
-  Pr[E_GAKE(Game2, A).run(true) @ &m : res]|)).
-smt(StdOrder.RealOrder.ler_norm_add).
-have : `|Pr[E_GAKE(Game2, A).run(false) @ &m : res] -
-  Pr[E_GAKE(Game2, A).run(true) @ &m : res]| <=
-`|Pr[E_GAKE(Game3, A).run(false) @ &m : res] -
-  Pr[E_GAKE(Game7, A).run(false) @ &m : res]| +
-`|Pr[E_GAKE(Game3, A).run(true) @ &m : res] -
-  Pr[E_GAKE(Game7, A).run(true) @ &m : res]| +
+        (`|Pr[AKE_Game(Game1a, A).run(false) @ &m : res] - Pr[AKE_Game(Game2, A).run(false) @ &m : res]| +
+         `|Pr[AKE_Game(Game1a, A).run(true) @ &m : res] - Pr[AKE_Game(Game2, A).run(true) @ &m : res]| +
+         `|Pr[AKE_Game(Game2, A).run(false) @ &m : res] - Pr[AKE_Game(Game2, A).run(true) @ &m : res]|)).
++ smt(StdOrder.RealOrder.ler_norm_add).
+have : `|Pr[AKE_Game(Game2, A).run(false) @ &m : res] -
+  Pr[AKE_Game(Game2, A).run(true) @ &m : res]| <=
+`|Pr[AKE_Game(Game3, A).run(false) @ &m : res] -
+  Pr[AKE_Game(Game5c, A).run(false) @ &m : res]| +
+`|Pr[AKE_Game(Game3, A).run(true) @ &m : res] -
+  Pr[AKE_Game(Game5c, A).run(true) @ &m : res]| +
 2%r * ((q_m1 + q_m2 + q_m3) ^ 2)%r * mu1 dctxt (mode dctxt); last by smt(StdOrder.RealOrder.ler_add2l).
 apply (StdOrder.RealOrder.ler_trans
-        (`|Pr[E_GAKE(Game3, A).run(false) @ &m : res] -
-  Pr[E_GAKE(Game3, A).run(true) @ &m : res]| +
+        (`|Pr[AKE_Game(Game3, A).run(false) @ &m : res] - Pr[AKE_Game(Game3, A).run(true) @ &m : res]| +
 2%r * ((q_m1 + q_m2 + q_m3) ^ 2)%r * mu1 dctxt (mode dctxt)
-)); 1: by smt(StdOrder.RealOrder.ler_norm_add Step2 Step2b).
+)); 1: by smt(StdOrder.RealOrder.ler_norm_add Hop4 Hop4_bound).
 rewrite StdOrder.RealOrder.ler_add2r.
-smt(StdOrder.RealOrder.ler_norm_add Step7 Step8).
+smt(StdOrder.RealOrder.ler_norm_add Hop14).
 qed.
